Refactor thread-local sim

src/axiomatic/PFtoA.v
@@ -19,43 +19,10 @@ Require Import PromisingArch.lib.Lang.
 Require Import PromisingArch.promising.Promising.
 Require Import PromisingArch.promising.StateExecFacts.
 Require Import PromisingArch.axiomatic.Axiomatic.
+Require Import PromisingArch.axiomatic.CommonAxiomatic.
 
 Set Implicit Arguments.
 
-
-Inductive inverse A (rel:relation A) (codom:A -> Prop) (a:A): Prop :=
-| inverse_intro
-    a'
-    (REL: rel a a')
-    (CODOM: codom a')
-.
-Hint Constructors inverse.
-
-Lemma inverse_mon A (r1 r2:relation A)
-      (REL: r1 ⊆ r2):
-  inverse r1 <2= inverse r2.
-Proof.
-  i. inv PR. econs; eauto.
-Qed.
-
-Lemma inverse_union A (r1 r2:relation A) s:
-  inverse (r1 ∪ r2) s = inverse r1 s \1/ inverse r2 s.
-Proof.
-  funext. i. propext. econs; i.
-  - inv H. inv REL; eauto.
-  - des; inv H; econs; eauto.
-    + left. ss.
-    + right. ss.
-Qed.
-
-Lemma inverse_step
-      r tid n:
-  inverse (r ⨾ Execution.po_adj) (eq (tid, S n)) = inverse r (eq (tid, n)).
-Proof.
-  funext. i. propext. econs; i.
-  - inv H. inv REL. des. inv H0. destruct x, x0. ss. inv N. econs; eauto.
-  - inv H. econs; eauto. econs; eauto.
-Qed.
 
 Definition sim_view (vext: eidT -> Time.t) (view: Time.t) (eids: eidT -> Prop): Prop :=
   forall eid (EID: eids eid), le (vext eid) view.
@@ -122,378 +89,6 @@ Proof.
     + ii. des. inv EID0.
       * etrans; [|eapply join_l]; eauto.
       * etrans; [|eapply join_r]; eauto.
-Qed.
-
-Definition sim_local_coh ex loc :=
-  ⦗ex.(Execution.label_is) (Label.is_writing loc)⦘ ⨾
-  ex.(Execution.rfe)^? ⨾
-  Execution.po.
-
-Lemma sim_local_coh_step ex loc:
-  sim_local_coh ex loc =
-  (sim_local_coh ex loc ∪
-   ⦗ex.(Execution.label_is) (Label.is_writing loc)⦘ ⨾ ex.(Execution.rfe)^?) ⨾
-  Execution.po_adj.
-Proof.
-  unfold sim_local_coh. rewrite Execution.po_po_adj at 1.
-  rewrite (clos_refl_union Execution.po), union_seq, eq_seq.
-  rewrite ? seq_union, ? union_seq, ? seq_assoc.
-  refl.
-Qed.
-
-Lemma sim_local_coh_spec
-      p ex loc eid1 eid2
-      (EX: Valid.ex p ex)
-      (EID2: Execution.label_is ex (Label.is_accessing loc) eid2)
-      (COH: sim_local_coh ex loc eid1 eid2):
-  <<INTERNAL: ex.(Execution.internal)⁺ eid1 eid2>> /\
-  <<LABEL: Execution.label_is ex (Label.is_writing loc) eid1>>.
-Proof.
-  inv COH. des. inv H. inv H0. des. inv EID2. inv H2. destruct l0; ss. inv H.
-  - esplits.
-    + econs. left. left. left. econs; eauto.
-    + destruct (equiv_dec loc0 loc); ss. inv e. econs; eauto. apply Label.write_is_writing.
-  - inv H1. splits.
-    + econs 2; [econs|].
-      { right. eauto. }
-      exploit EX.(Valid.RF2); eauto. i. des.
-      rewrite EID0 in WRITE. inv WRITE.
-      econs. left. left. left. econs; eauto.
-    + destruct (equiv_dec loc0 loc); ss. inv e. econs; eauto. apply Label.write_is_writing.
-Qed.
-
-Definition sim_local_vrp ex :=
-  (⦗ex.(Execution.label_is) Label.is_read⦘ ⨾
-   Execution.po ⨾
-   ⦗ex.(Execution.label_is) (Label.is_barrier_c Barrier.is_dmb_rr)⦘ ⨾
-   Execution.po) ∪
-
-  (⦗ex.(Execution.label_is) Label.is_write⦘ ⨾
-   Execution.po ⨾
-   ⦗ex.(Execution.label_is) (Label.is_barrier_c Barrier.is_dmb_wr)⦘ ⨾
-   Execution.po) ∪
-
-  ((ex.(Execution.ctrl) ∪ (ex.(Execution.addr) ⨾ Execution.po)) ⨾
-   ⦗ex.(Execution.label_is) (eq (Label.barrier Barrier.isb))⦘ ⨾
-   Execution.po) ∪
-
-  (⦗ex.(Execution.label_is) (Label.is_acquire_pc)⦘ ⨾
-   Execution.po).
-
-Lemma sim_local_vrp_step ex:
-  sim_local_vrp ex =
-  (sim_local_vrp ex ∪
-   ((⦗ex.(Execution.label_is) Label.is_read⦘ ⨾
-     Execution.po ⨾
-     ⦗ex.(Execution.label_is) (Label.is_barrier_c Barrier.is_dmb_rr)⦘) ∪
-
-   (⦗ex.(Execution.label_is) Label.is_write⦘ ⨾
-     Execution.po ⨾
-     ⦗ex.(Execution.label_is) (Label.is_barrier_c Barrier.is_dmb_wr)⦘) ∪
-
-    ((ex.(Execution.ctrl) ∪ (ex.(Execution.addr) ⨾ Execution.po)) ⨾
-     ⦗ex.(Execution.label_is) (eq (Label.barrier Barrier.isb))⦘) ∪
-
-    (⦗ex.(Execution.label_is) (Label.is_acquire_pc)⦘))) ⨾
-  Execution.po_adj.
-Proof.
-  unfold sim_local_vrp. rewrite ? (union_seq' Execution.po_adj), ? seq_assoc, ? union_assoc.
-  rewrite Execution.po_po_adj at 2 4 6 7.
-  rewrite (clos_refl_union Execution.po), union_seq, eq_seq.
-  rewrite ? (seq_union' (Execution.po ⨾ Execution.po_adj) Execution.po_adj), ? seq_assoc, ? union_assoc.
-  funext. i. funext. i. propext. econs; i.
-  - repeat match goal with
-           | [H: (_ ∪ _) _ _ |- _] => inv H
-           end;
-      eauto 10 using union_l, union_r.
-  - repeat match goal with
-           | [H: (_ ∪ _) _ _ |- _] => inv H
-           end;
-      eauto 10 using union_l, union_r.
-Qed.
-
-Lemma sim_local_vrp_spec
-      p ex eid1 eid2
-      (EX: Valid.ex p ex)
-      (EID2: Execution.label_is ex Label.is_read eid2)
-      (VRP: sim_local_vrp ex eid1 eid2):
-  <<OB: ex.(Execution.ob) eid1 eid2>>.
-Proof.
-  inv EID2. destruct l; inv LABEL. unfold sim_local_vrp in VRP.
-  repeat match goal with
-         | [H: (_ ∪ _) _ _ |- _] => inv H
-         end.
-  - right. left. left. left. left. left. left. left.
-    inv H. des. econs. splits; eauto.
-    rewrite ? seq_assoc. econs. splits; [|by econs; eauto].
-    rewrite <- ? seq_assoc. ss.
-  - right. left. left. left. left. left. right.
-    inv H. des. econs. splits; eauto.
-    rewrite ? seq_assoc. econs. splits; [|by econs; eauto].
-    rewrite <- ? seq_assoc. ss.
-  - left. left. right. right.
-    inv H0. des. econs. splits; eauto.
-    right. rewrite seq_assoc. econs. splits; eauto. econs; ss. econs; eauto.
-  - right. left. left. right.
-    inv H. des. econs. splits; eauto.
-Qed.
-
-Definition sim_local_vwp ex :=
-  (⦗ex.(Execution.label_is) Label.is_read⦘ ⨾
-   Execution.po ⨾
-   ⦗ex.(Execution.label_is) (Label.is_barrier_c Barrier.is_dmb_rw)⦘ ⨾
-   Execution.po) ∪
-
-  (⦗ex.(Execution.label_is) Label.is_write⦘ ⨾
-   Execution.po ⨾
-   ⦗ex.(Execution.label_is) (Label.is_barrier_c Barrier.is_dmb_ww)⦘ ⨾
-   Execution.po) ∪
-
-  (⦗ex.(Execution.label_is) (Label.is_acquire_pc)⦘ ⨾
-   Execution.po).
-
-Lemma sim_local_vwp_step ex:
-  sim_local_vwp ex =
-  (sim_local_vwp ex ∪
-   ((⦗ex.(Execution.label_is) Label.is_read⦘ ⨾
-     Execution.po ⨾
-     ⦗ex.(Execution.label_is) (Label.is_barrier_c Barrier.is_dmb_rw)⦘) ∪
-
-   (⦗ex.(Execution.label_is) Label.is_write⦘ ⨾
-     Execution.po ⨾
-     ⦗ex.(Execution.label_is) (Label.is_barrier_c Barrier.is_dmb_ww)⦘) ∪
-
-    (⦗ex.(Execution.label_is) (Label.is_acquire_pc)⦘))) ⨾
-  Execution.po_adj.
-Proof.
-  unfold sim_local_vwp. rewrite ? (union_seq' Execution.po_adj), ? seq_assoc, ? union_assoc.
-  rewrite Execution.po_po_adj at 2 4 5.
-  rewrite (clos_refl_union Execution.po), union_seq, eq_seq.
-  rewrite ? (seq_union' (Execution.po ⨾ Execution.po_adj) Execution.po_adj), ? seq_assoc, ? union_assoc.
-  funext. i. funext. i. propext. econs; i.
-  - repeat match goal with
-           | [H: (_ ∪ _) _ _ |- _] => inv H
-           end;
-      eauto 10 using union_l, union_r.
-  - repeat match goal with
-           | [H: (_ ∪ _) _ _ |- _] => inv H
-           end;
-      eauto 10 using union_l, union_r.
-Qed.
-
-Lemma sim_local_vwp_spec
-      p ex eid1 eid2
-      (EX: Valid.ex p ex)
-      (EID2: Execution.label_is ex Label.is_write eid2)
-      (VWP: sim_local_vwp ex eid1 eid2):
-  <<OB: ex.(Execution.ob) eid1 eid2>>.
-Proof.
-  inv EID2. destruct l; inv LABEL. unfold sim_local_vwp in VWP.
-  repeat match goal with
-         | [H: (_ ∪ _) _ _ |- _] => inv H
-         end.
-  - right. left. left. left. left. left. left. right.
-    inv H0. des. econs. splits; eauto.
-    rewrite ? seq_assoc. econs. splits; [|by econs; eauto].
-    rewrite <- ? seq_assoc. ss.
-  - right. left. left. left. left. right.
-    inv H0. des. econs. splits; eauto.
-    rewrite ? seq_assoc. econs. splits; [|by econs; eauto].
-    rewrite <- ? seq_assoc. ss.
-  - right. left. left. right.
-    inv H. des. econs. splits; eauto.
-Qed.
-
-Definition sim_local_vrm ex :=
-  ⦗ex.(Execution.label_is) (Label.is_read)⦘ ⨾ Execution.po.
-
-Lemma sim_local_vrm_step ex:
-  sim_local_vrm ex =
-  (sim_local_vrm ex ∪ ⦗ex.(Execution.label_is) (Label.is_read)⦘) ⨾
-  Execution.po_adj.
-Proof.
-  unfold sim_local_vrm. rewrite ? (union_seq' Execution.po_adj), ? seq_assoc, ? union_assoc.
-  rewrite Execution.po_po_adj at 1.
-  rewrite (clos_refl_union Execution.po), union_seq, eq_seq.
-  rewrite ? (seq_union' (Execution.po ⨾ Execution.po_adj) Execution.po_adj), ? seq_assoc, ? union_assoc.
-  refl.
-Qed.
-
-Definition sim_local_vwm ex :=
-  ⦗ex.(Execution.label_is) (Label.is_write)⦘ ⨾ Execution.po.
-
-Lemma sim_local_vwm_step ex:
-  sim_local_vwm ex =
-  (sim_local_vwm ex ∪ ⦗ex.(Execution.label_is) (Label.is_write)⦘) ⨾
-  Execution.po_adj.
-Proof.
-  unfold sim_local_vwm. rewrite ? (union_seq' Execution.po_adj), ? seq_assoc, ? union_assoc.
-  rewrite Execution.po_po_adj at 1.
-  rewrite (clos_refl_union Execution.po), union_seq, eq_seq.
-  rewrite ? (seq_union' (Execution.po ⨾ Execution.po_adj) Execution.po_adj), ? seq_assoc, ? union_assoc.
-  refl.
-Qed.
-
-Definition sim_local_vcap ex :=
-  ex.(Execution.ctrl) ∪ (ex.(Execution.addr) ⨾ Execution.po).
-
-Lemma sim_local_vcap_po
-      p ex
-      (EX: Valid.ex p ex):
-  (sim_local_vcap ex ⨾ Execution.po) ⊆ sim_local_vcap ex.
-Proof.
-  unfold sim_local_vcap. ii. inv H. des. inv H0.
-  - left. eapply Valid.ctrl_po; eauto. econs. splits; eauto.
-  - right. inv H. des. econs. splits; eauto. etrans; eauto.
-Qed.
-
-Lemma sim_local_vcap_po_adj
-      p ex
-      (EX: Valid.ex p ex):
-  (sim_local_vcap ex ⨾ Execution.po_adj) ⊆ sim_local_vcap ex.
-Proof.
-  ii. eapply sim_local_vcap_po; eauto.
-  inv H. des. econs. splits; eauto. apply Execution.po_adj_po. ss.
-Qed.
-
-Definition sim_local_vrel ex :=
-  ⦗ex.(Execution.label_is) (Label.is_release)⦘ ⨾ Execution.po.
-
-Lemma sim_local_vrel_step ex:
-  sim_local_vrel ex =
-  (sim_local_vrel ex ∪ ⦗ex.(Execution.label_is) (Label.is_release)⦘) ⨾
-  Execution.po_adj.
-Proof.
-  unfold sim_local_vrel. rewrite ? (union_seq' Execution.po_adj), ? seq_assoc, ? union_assoc.
-  rewrite Execution.po_po_adj at 1.
-  rewrite (clos_refl_union Execution.po), union_seq, eq_seq.
-  rewrite ? (seq_union' (Execution.po ⨾ Execution.po_adj) Execution.po_adj), ? seq_assoc, ? union_assoc.
-  refl.
-Qed.
-
-Lemma sim_local_vrel_spec
-      p ex eid1 eid2
-      (EX: Valid.ex p ex)
-      (EID2: Execution.label_is ex Label.is_acquire eid2)
-      (VREL: sim_local_vrel ex eid1 eid2):
-  <<OB: ex.(Execution.ob) eid1 eid2>>.
-Proof.
-  inv EID2. destruct l; inv LABEL. unfold sim_local_vrel in VREL.
-  right. left. left. left. right.
-  rewrite seq_assoc. econs. splits; eauto. econs; eauto.
-Qed.
-
-Inductive sim_local_fwd ex (loc:Loc.t) (eid1 eid2:eidT): Prop :=
-| sim_local_fwd_intro
-    (PO: Execution.po eid1 eid2)
-    (WRITE: ex.(Execution.label_is) (Label.is_writing loc) eid1)
-    (NWRITE: forall eid
-               (PO: Execution.po eid1 eid)
-               (PO: Execution.po eid eid2),
-        ex.(Execution.label_is) (fun l => ~ Label.is_writing loc l) eid)
-.
-
-Lemma sim_local_fwd_step ex loc:
-  sim_local_fwd ex loc =
-  (sim_local_fwd ex loc ⨾ ⦗ex.(Execution.label_is) (fun l => ~ (Label.is_writing loc l))⦘ ∪
-   ⦗ex.(Execution.label_is) (Label.is_writing loc)⦘) ⨾
-  Execution.po_adj.
-Proof.
-  funext. i. funext. i. propext. econs.
-  - i. inv H. rewrite Execution.po_po_adj in PO. inv PO. des.
-    inv H0. destruct x0, x1. ss. subst.
-    econs. splits; cycle 1.
-    { instantiate (1 := (_, _)). econs; ss. }
-    inv H.
-    + right. econs; ss.
-    + hexploit NWRITE; eauto. i.
-      left. econs. splits; cycle 1.
-      { econs; eauto. }
-      econs; eauto. i. apply NWRITE; eauto. etrans; eauto.
-  - i. inv H. des. inv H1. destruct x0, x1. ss. subst. inv H0.
-    + inv H. des. inv H1. inv H2. inv H0.
-      econs; eauto.
-      * etrans; eauto.
-      * i. rewrite Execution.po_po_adj in PO1. inv PO1. des. inv H0. destruct x0. ss. inv N.
-        inv H; eauto.
-    + inv H. inv H1. apply Label.is_writing_inv in LABEL. des. subst.
-      econs; eauto.
-      * econs; eauto. apply Label.write_is_writing.
-      * i. inv PO. inv PO0. ss. subst. lia.
-Qed.
-
-Lemma sim_local_fwd_functional ex loc eid1 eid2 eid3
-      (EID1: sim_local_fwd ex loc eid1 eid3)
-      (EID2: sim_local_fwd ex loc eid2 eid3):
-  eid1 = eid2.
-Proof.
-  inv EID1. inv EID2.
-  destruct eid1, eid2, eid3. inv PO. inv PO0. ss. subst. f_equal.
-  destruct (Nat.compare_spec n n0); ss.
-  - exploit (NWRITE (t1, n0)); eauto. i.
-    inv WRITE0. apply Label.is_writing_inv in LABEL. des. subst.
-    inv x0. rewrite EID in EID0. inv EID0. ss. destruct (equiv_dec loc loc); ss. congr.
-  - exploit (NWRITE0 (t1, n)); eauto. i.
-    inv WRITE. apply Label.is_writing_inv in LABEL. des. subst.
-    inv x0. rewrite EID in EID0. inv EID0. ss. destruct (equiv_dec loc loc); ss. congr.
-Qed.
-
-Lemma rfi_sim_local_fwd
-      p ex (EX: Valid.ex p ex)
-      loc eid1 eid2
-      (EID1: ex.(Execution.label_is) (Label.is_writing loc) eid1)
-      (EID2: ex.(Execution.label_is) (Label.is_reading loc) eid2)
-      (RFI: ex.(Execution.rfi) eid1 eid2):
-  sim_local_fwd ex loc eid1 eid2.
-Proof.
-  destruct eid1 as [tid1 n1].
-  destruct eid2 as [tid2 n2].
-  inv RFI. inv H0. ss. subst.
-  destruct (Nat.compare_spec n1 n2).
-  - subst. exfalso. eapply EX.(Valid.INTERNAL).
-    econs. right. eauto.
-  - econs; ss. i. destruct eid. inv PO. inv PO0. ss. subst.
-    inv EID1. apply Label.is_writing_inv in LABEL. des. subst.
-    inv EID2. apply Label.is_reading_inv in LABEL. des. subst.
-    exploit Valid.po_label; eauto.
-    { instantiate (1 := (t, n)). econs; ss. }
-    i. des. econs; eauto. intro X. apply Label.is_writing_inv in X. des. subst.
-    exploit Valid.coherence_ww.
-    { eauto. }
-    { econs; try exact EID; eauto. apply Label.write_is_writing. }
-    { econs; try exact LABEL; eauto. apply Label.write_is_writing. }
-    { econs; ss. }
-    i.
-    exploit Valid.coherence_wr; try exact H; eauto.
-    { econs; try exact LABEL; eauto. apply Label.write_is_writing. }
-    { econs; try exact EID0; eauto. apply Label.read_is_reading. }
-    { econs; ss. }
-    i. des.
-    exploit EX.(Valid.RF_WF); [exact H|exact RF|]. i. subst.
-    inv CO.
-    + inv H1. lia.
-    + exfalso. eapply EX.(Valid.INTERNAL). econs 2; econs; left; right; eauto.
-  - exfalso. eapply EX.(Valid.INTERNAL). econs 2; [econs|econs].
-    + right. eauto.
-    + left. left. left. econs; eauto.
-      inv EID1. apply Label.is_writing_inv in LABEL. des. subst.
-      inv EID2. apply Label.is_reading_inv in LABEL. des. subst.
-      econs; eauto. econs; eauto using Label.read_is_accessing, Label.write_is_accessing.
-Qed.
-
-Definition sim_local_fwd_none ex loc :=
-  ⦗ex.(Execution.label_is) (Label.is_writing loc)⦘ ⨾ Execution.po.
-
-Lemma sim_local_fwd_none_step ex loc:
-  sim_local_fwd_none ex loc =
-  (sim_local_fwd_none ex loc ∪ ⦗ex.(Execution.label_is) (Label.is_writing loc)⦘) ⨾
-  Execution.po_adj.
-Proof.
-  unfold sim_local_fwd_none. rewrite ? (union_seq' Execution.po_adj), ? seq_assoc, ? union_assoc.
-  rewrite Execution.po_po_adj at 1.
-  rewrite (clos_refl_union Execution.po), union_seq, eq_seq.
-  rewrite ? (seq_union' (Execution.po ⨾ Execution.po_adj) Execution.po_adj), ? seq_assoc, ? union_assoc.
-  refl.
 Qed.
 
 Inductive sim_local (tid:Id.t) (ex: Execution.t) (vext: eidT -> Time.t) (local:Local.t (A:=unit)) (alocal:ALocal.t): Prop := mk_sim_local {
@@ -564,192 +159,6 @@ Inductive sim_eu (tid:Id.t) (ex:Execution.t) (vext: eidT -> Time.t) (eu:ExecUnit
     (LOCAL: sim_local tid ex vext eu.(ExecUnit.local) aeu.(AExecUnit.local))
 .
 Hint Constructors sim_eu.
-
-(* Lemma label_read_mem_of_ex *)
-(*       eid ex ob exm ord loc val *)
-(*       (OB: Permutation ob (Execution.eids ex)) *)
-(*       (LABEL: Execution.label eid ex = Some (Label.read exm ord loc val)): *)
-(*   exists view, *)
-(*     <<VIEW: view_of_eid ex ob eid = Some view>>. *)
-(* Proof. *)
-(*   generalize (Execution.eids_spec ex). i. des. rename NODUP into NODUP0. *)
-(*   specialize (LABEL0 eid). rewrite LABEL in LABEL0. *)
-(*   inv LABEL0. clear H0. exploit H; [congr|]. clear H. intro IN0. *)
-(*   symmetry in OB. exploit Permutation_in; eauto. intro IN. *)
-(*   exploit HahnList.Permutation_nodup; eauto. intro NODUP. *)
-(*   generalize (List_in_find_pos _ ob IN). i. des. *)
-(*   unfold view_of_eid. rewrite H. s. eauto. *)
-(* Qed. *)
-
-(* Lemma label_write_mem_of_ex_msg *)
-(*       eid ex ob exm ord loc val *)
-(*       (OB: Permutation ob (Execution.eids ex)) *)
-(*       (LABEL: Execution.label eid ex = Some (Label.write exm ord loc val)): *)
-(*   exists n, *)
-(*     <<VIEW: view_of_eid ex ob eid = Some (S n)>> /\ *)
-(*     <<MSG: List.nth_error (mem_of_ex ex ob) n = Some (Msg.mk loc val eid.(fst))>>. *)
-(* Proof. *)
-(*   generalize (Execution.eids_spec ex). i. des. rename NODUP into NODUP0. *)
-(*   specialize (LABEL0 eid). rewrite LABEL in LABEL0. *)
-(*   inv LABEL0. clear H0. exploit H; [congr|]. clear H. intro IN0. *)
-(*   symmetry in OB. exploit Permutation_in; eauto. intro IN. *)
-(*   exploit HahnList.Permutation_nodup; eauto. intro NODUP. *)
-(*   generalize (List_in_find_pos _ ob IN). i. des. *)
-(*   unfold view_of_eid. rewrite H. *)
-(*   exploit List_find_pos_inv; eauto. i. des. *)
-(*   destruct (equiv_dec a eid); [|done]. inversion e. subst. *)
-(*   esplits. *)
-(*   - unfold option_map. erewrite List_firstn_S; eauto. *)
-(*     rewrite mem_of_ex_app, List.app_length. *)
-(*     unfold mem_of_ex at 2. s. rewrite LABEL. s. rewrite Nat.add_1_r. ss. *)
-(*   - rewrite <- (List.firstn_skipn n ob) at 1. *)
-(*     rewrite mem_of_ex_app, List.nth_error_app2; [|lia]. *)
-(*     erewrite Nat.sub_diag, List_skipn_cons; eauto. s. *)
-(*     unfold mem_of_ex. s. rewrite LABEL. ss. *)
-(* Qed. *)
-
-(* Lemma label_write_mem_of_ex *)
-(*       eid ex ob exm ord loc val *)
-(*       (OB: Permutation ob (Execution.eids ex)) *)
-(*       (LABEL: Execution.label eid ex = Some (Label.write exm ord loc val)): *)
-(*   exists n, *)
-(*     <<VIEW: view_of_eid ex ob eid = Some (S n)>> /\ *)
-(*     <<READ: Memory.read loc (S n) (mem_of_ex ex ob) = Some val>> /\ *)
-(*     <<MSG: Memory.get_msg (S n) (mem_of_ex ex ob) = Some (Msg.mk loc val eid.(fst))>>. *)
-(* Proof. *)
-(*   exploit label_write_mem_of_ex_msg; eauto. i. des. *)
-(*   esplits; eauto. *)
-(*   unfold Memory.read. s. rewrite MSG. s. condtac; [|congr]. ss. *)
-(* Qed. *)
-
-(* Lemma in_mem_of_ex *)
-(*       ex ob view msg *)
-(*       (NODUP: List.NoDup ob) *)
-(*       (IN: List.nth_error (mem_of_ex ex ob) view = Some msg): *)
-(*   exists n ex1 ord1, *)
-(*     <<LABEL: Execution.label (msg.(Msg.tid), n) ex = Some (Label.write ex1 ord1 msg.(Msg.loc) msg.(Msg.val))>> /\ *)
-(*     <<VIEW: view_of_eid ex ob (msg.(Msg.tid), n) = Some (S view)>>. *)
-(* Proof. *)
-(*   unfold mem_of_ex in IN. exploit nth_error_filter_map_inv; eauto. i. des. *)
-(*   destruct (Execution.label a ex) eqn:LABEL; ss. destruct t; inv FA. destruct a. ss. *)
-(*   esplits. *)
-(*   - eauto. *)
-(*   - unfold view_of_eid. *)
-(*     erewrite List_nth_error_find_pos; eauto. s. f_equal. ss. *)
-(* Qed. *)
-
-Definition promises_from_mem
-           (tid:Id.t) (mem: Memory.t): Promises.t.
-Proof.
-  induction mem using list_rev_rect.
-  - exact bot.
-  - destruct x.
-    apply (if tid0 == tid
-           then Promises.set (S (List.length (List.rev mem))) IHmem
-           else IHmem).
-Defined.
-
-Lemma promises_from_mem_nil tid:
-  promises_from_mem tid Memory.empty = bot.
-Proof.
-  unfold promises_from_mem, list_rev_rect, eq_rect. ss.
-  match goal with
-  | [|- context[match ?c with | eq_refl => _ end]] => destruct c
-  end; ss.
-Qed.
-
-Lemma promises_from_mem_snoc tid mem msg:
-  promises_from_mem tid (mem ++ [msg]) =
-  if msg.(Msg.tid) == tid
-  then Promises.set (S (List.length mem)) (promises_from_mem tid mem)
-  else promises_from_mem tid mem.
-Proof.
-  unfold promises_from_mem at 1, list_rev_rect, eq_rect.
-  match goal with
-  | [|- context[match ?c with | eq_refl => _ end]] => destruct c
-  end; ss.
-  rewrite List.rev_involutive, List.rev_app_distr. ss.
-  destruct msg. s. condtac.
-  - inversion e. subst. rewrite ? List.rev_length.
-    f_equal.
-    unfold promises_from_mem, list_rev_rect, eq_rect.
-    match goal with
-    | [|- context[match ?c with | eq_refl => _ end]] => destruct c
-    end; ss.
-  - unfold promises_from_mem, list_rev_rect, eq_rect.
-    match goal with
-    | [|- context[match ?c with | eq_refl => _ end]] => destruct c
-    end; ss.
-Qed.
-
-Lemma promises_from_mem_inv
-      ts tid mem
-      (LOOKUP: Promises.lookup (S ts) (promises_from_mem tid mem)):
-  exists loc val, List.nth_error mem ts = Some (Msg.mk loc val tid).
-Proof.
-  revert LOOKUP. induction mem using List.rev_ind.
-  { rewrite promises_from_mem_nil, Promises.lookup_bot. ss. }
-  rewrite promises_from_mem_snoc. condtac.
-  { rewrite Promises.set_o. condtac.
-    - inversion e. inversion e0. subst.
-      rewrite List.nth_error_app2; [|lia].
-      rewrite Nat.sub_diag. ss.
-      destruct x. esplits; eauto.
-    - i. exploit IHmem; eauto.  i. des.
-      rewrite List.nth_error_app1; eauto.
-      apply List.nth_error_Some. congr.
-  }
-  i. exploit IHmem; eauto.  i. des.
-  rewrite List.nth_error_app1; eauto.
-  apply List.nth_error_Some. congr.
-Qed.
-
-Definition init_with_promises (p:program) (mem:Memory.t): Machine.t :=
-  Machine.mk
-    (IdMap.mapi (fun tid stmts =>
-                   (State.init stmts,
-                    Local.init_with_promises (promises_from_mem tid mem)))
-                p)
-    mem.
-
-Lemma pf_init_with_promises
-      p promises
-      (MEM: forall msg (MSG: List.In msg promises), IdMap.find msg.(Msg.tid) p <> None):
-  exists m,
-    <<STEP: rtc (Machine.step ExecUnit.promise_step) (Machine.init p) m>> /\
-    <<TPOOL: IdMap.Equal m.(Machine.tpool) (init_with_promises p promises).(Machine.tpool)>> /\
-    <<MEM: m.(Machine.mem) = promises>>.
-Proof.
-  revert MEM. induction promises using List.rev_ind; i.
-  { esplits; eauto. ii. s. rewrite IdMap.map_spec, IdMap.mapi_spec.
-    destruct (IdMap.find y p); ss.
-    unfold Local.init, Local.init_with_promises. repeat f_equal.
-    rewrite promises_from_mem_nil. ss.
-  }
-  exploit IHpromises; eauto.
-  { i. apply MEM. apply List.in_app_iff. intuition. }
-  i. des. subst. destruct x.
-  hexploit MEM.
-  { apply List.in_app_iff. right. left. eauto. }
-  match goal with
-  | [|- context[(?f <> None) -> _]] => destruct f eqn:FIND
-  end; ss.
-  intro X. clear X.
-  eexists (Machine.mk _ _). esplits.
-  - etrans; [eauto|]. econs 2; [|refl].
-    econs.
-    + rewrite TPOOL, IdMap.mapi_spec, FIND. ss.
-    + econs; ss. econs; eauto. ss.
-    + ss.
-  - s. ii. rewrite IdMap.add_spec. condtac; ss.
-    + inversion e. subst. rewrite IdMap.mapi_spec, FIND. s.
-      unfold Local.init_with_promises. repeat f_equal.
-      rewrite promises_from_mem_snoc. condtac; ss.
-    + rewrite TPOOL, ? IdMap.mapi_spec. destruct (IdMap.find y p); ss.
-      unfold Local.init_with_promises. rewrite promises_from_mem_snoc. s.
-      condtac; ss. congr.
-  - ss.
-Qed.
 
 Inductive sim_val_weak (vala:ValA.t (A:=View.t (A:=unit))) (avala:ValA.t (A:=nat -> Prop)): Prop :=
 | sim_val_weak_intro
@@ -912,28 +321,6 @@ Proof.
   induction SIM; ss. des. splits; congr.
 Qed.
 
-(* TODO: move *)
-  Lemma step_get_msg_tpool
-        p m ts msg
-        (STEPS: rtc (Machine.step ExecUnit.step) (Machine.init p) m)
-        (MSG: Memory.get_msg ts m.(Machine.mem) = Some msg):
-    exists sl, IdMap.find msg.(Msg.tid) m.(Machine.tpool) = Some sl.
-  Proof.
-    apply clos_rt_rt1n_iff in STEPS.
-    apply clos_rt_rtn1_iff in STEPS.
-    revert ts msg MSG. induction STEPS; ss.
-    { destruct ts; ss. destruct ts; ss. }
-    destruct y as [tpool1 mem1].
-    destruct z as [tpool2 mem2].
-    ss. inv H. ss. i. inv STEP.
-    - rewrite IdMap.add_spec. condtac; eauto.
-      inv STEP0. inv STEP. ss. subst. eauto.
-    - rewrite IdMap.add_spec. condtac; eauto.
-      inv STEP0. ss. subst. inv LOCAL. inv MEM2.
-      apply Memory.get_msg_snoc_inv in MSG. des; eauto. subst.
-      ss. congr.
-  Qed.
-
 Lemma sim_traces_memory
       p trs atrs rs ws covs vexts
       m
@@ -957,28 +344,6 @@ Proof.
   - s. i. des. inv EQUIV. generalize (TPOOL tid). congr.
 Qed.
 
-(* TODO: move *)
-  Lemma rtc_promise_step_spec
-        p m
-        (STEP: rtc (Machine.step ExecUnit.promise_step) (Machine.init p) m):
-    IdMap.Equal m.(Machine.tpool) (init_with_promises p m.(Machine.mem)).(Machine.tpool).
-  Proof.
-    apply clos_rt_rt1n_iff in STEP.
-    apply clos_rt_rtn1_iff in STEP.
-    induction STEP.
-    { s. ii. rewrite IdMap.map_spec, IdMap.mapi_spec.
-      destruct (IdMap.find y p); ss. f_equal. f_equal.
-      rewrite promises_from_mem_nil. ss.
-    }
-    destruct y as [tpool2 mem2].
-    destruct z as [tpool3 mem3].
-    ss. inv H. inv STEP0. inv LOCAL. ss. subst. inv MEM2.
-    ii. generalize (IHSTEP y). rewrite IdMap.add_spec, ? IdMap.mapi_spec.
-    rewrite promises_from_mem_snoc. s.
-    repeat condtac; try congr.
-    inversion e. subst. rewrite FIND. destruct (IdMap.find tid p); ss. i. inv H. ss.
-  Qed.
-
 Ltac simplify :=
   repeat
     (try match goal with
@@ -991,7 +356,6 @@ Ltac simplify :=
          | [H: Some _ = Some _ |- _] => inv H
          | [H: _::_ = _::_ |- _] => inv H
          end).
-
 
 Lemma promising_pf_sim_step
       tid e (eu1 eu2:ExecUnit.t (A:=unit)) aeu1
@@ -1174,145 +538,6 @@ all: ss.
 1: { apply bot. (* it's ex's rf. *) }
 Qed.      
 
-Lemma w_property
-      p mem tid tr atr wl rl covl vextl
-      (SIM: sim_trace p mem tid tr atr wl rl covl vextl):
-  exists eu tr' aeu atr' w wl',
-    tr = eu :: tr' /\
-    atr = aeu :: atr' /\
-    wl = w :: wl' /\
-    <<WPROP1:
-      forall ts loc val
-         (GET: Memory.get_msg ts mem = Some (Msg.mk loc val tid)),
-        ((Promises.lookup ts eu.(ExecUnit.local).(Local.promises) = true /\
-          forall eid, w eid <> Some (loc, ts)) \/
-         (Promises.lookup ts eu.(ExecUnit.local).(Local.promises) = false /\
-          exists eid ex ord,
-            w eid = Some (loc, ts) /\
-            List.nth_error aeu.(AExecUnit.local).(ALocal.labels) eid = Some (Label.write ex ord loc val)))>> /\
-    <<WPROP2:
-      forall eid ex ord loc val
-        (GET: List.nth_error aeu.(AExecUnit.local).(ALocal.labels) eid = Some (Label.write ex ord loc val)),
-      exists ts,
-        w eid = Some (loc, ts) /\
-        Memory.get_msg ts mem = Some (Msg.mk loc val tid)>> /\
-    <<WPROP3:
-      forall eid loc ts (GET: w eid = Some (loc, ts)),
-        Time.lt Time.bot ts /\
-      exists ex ord val,
-        List.nth_error aeu.(AExecUnit.local).(ALocal.labels) eid = Some (Label.write ex ord loc val) /\
-        Memory.get_msg ts mem = Some (Msg.mk loc val tid)>> /\
-    <<WPROP4:
-      forall eid1 loc1 eid2 loc2 ts (W1: w eid1 = Some (loc1, ts)) (W2: w eid2 = Some (loc2, ts)),
-        eid1 = eid2>>.
-Proof.
-  induction SIM.
-  { esplits; ss.
-    - rewrite IdMap.mapi_spec, STMT in FIND. inv FIND. s. i.
-      left. splits; ss. admit. (* promises_from_mem *)
-    - rewrite IdMap.mapi_spec, STMT in FIND. inv FIND. s. i.
-      destruct eid; ss.
-  }
-  des. simplify.
-  destruct eu as [st1 lc1 mem1].
-  destruct eu2 as [st2 lc2 mem2].
-  destruct aeu2 as [ast2 alc2].
-  ss. inv STEP. inv EVENT; inv LOCAL; inv EVENT; ss.
-  - (* internal *)
-    inv LC. s. inv ALOCAL_STEP; inv EVENT; ss. esplits; eauto.
-  - (* read *)
-    inv STEP; ss. inv ALOCAL_STEP; inv EVENT; ss. esplits; ss. all: ss.
-    + i. exploit WPROP1; eauto. i. des; [left|right]; esplits; eauto.
-      eapply nth_error_app_mon. eauto.
-    + i. exploit WPROP2; eauto.
-      apply nth_error_app_inv in GET. des; eauto.
-      apply nth_error_singleton_inv in GET0. des. congr.
-    + i. exploit WPROP3; eauto. i. des. esplits; eauto.
-      eapply nth_error_app_mon. eauto.
-  - (* write *)
-    admit.
-  - (* write failure *)
-    inv STEP; ss. inv ALOCAL_STEP; inv EVENT; ss. esplits; eauto.
-  - (* isb *)
-    inv STEP; ss. inv ALOCAL_STEP; inv EVENT; ss. esplits; ss. all: ss.
-    + i. exploit WPROP1; eauto. i. des; [left|right]; esplits; eauto.
-      eapply nth_error_app_mon. eauto.
-    + i. exploit WPROP2; eauto.
-      apply nth_error_app_inv in GET. des; eauto.
-      apply nth_error_singleton_inv in GET0. des. congr.
-    + i. exploit WPROP3; eauto. i. des. esplits; eauto.
-      eapply nth_error_app_mon. eauto.
-  - (* dmb *)
-    inv STEP; ss. inv ALOCAL_STEP; inv EVENT; ss. esplits; ss. all: ss.
-    + i. exploit WPROP1; eauto. i. des; [left|right]; esplits; eauto.
-      eapply nth_error_app_mon. eauto.
-    + i. exploit WPROP2; eauto.
-      apply nth_error_app_inv in GET. des; eauto.
-      apply nth_error_singleton_inv in GET0. des. congr.
-    + i. exploit WPROP3; eauto. i. des. esplits; eauto.
-      eapply nth_error_app_mon. eauto.
-Admitted.
-
-Lemma r_property
-      p mem tid tr atr wl rl covl vextl
-      (SIM: sim_trace p mem tid tr atr wl rl covl vextl):
-  exists eu tr' aeu atr' r rl',
-    tr = eu :: tr' /\
-    atr = aeu :: atr' /\
-    rl = r :: rl' /\
-    <<RPROP1:
-      forall eid ex ord loc val
-         (GET: List.nth_error aeu.(AExecUnit.local).(ALocal.labels) eid = Some (Label.read ex ord loc val)),
-      exists ts tid',
-        r eid = Some (loc, ts) /\
-        __guard__ ((ts = Time.bot /\ val = Val.default) \/
-         Memory.get_msg ts mem = Some (Msg.mk loc val tid'))>> /\
-    <<RPROP2:
-      forall eid loc ts (GET: r eid = Some (loc, ts)),
-      exists ex ord val tid',
-        List.nth_error aeu.(AExecUnit.local).(ALocal.labels) eid = Some (Label.read ex ord loc val) /\
-        __guard__ ((ts = Time.bot /\ val = Val.default) \/
-         Memory.get_msg ts mem = Some (Msg.mk loc val tid'))>>.
-Proof.
-  induction SIM.
-  { esplits; ss.
-    rewrite IdMap.mapi_spec, STMT in FIND. inv FIND. s. i.
-    destruct eid; ss.
-  }
-  des. simplify.
-  destruct eu as [st1 lc1 mem1].
-  destruct eu2 as [st2 lc2 mem2].
-  destruct aeu2 as [ast2 alc2].
-  ss. inv STEP. inv EVENT; inv LOCAL; inv EVENT; ss.
-  - (* internal *)
-    inv LC. s. inv ALOCAL_STEP; inv EVENT; ss. esplits; eauto.
-  - (* read *)
-    admit.
-  - (* write *)
-    inv STEP; ss. inv ALOCAL_STEP; inv EVENT; ss. esplits; ss. all: ss.
-    + i. exploit RPROP1; eauto.
-      apply nth_error_app_inv in GET. des; eauto.
-      apply nth_error_singleton_inv in GET0. des. congr.
-    + i. exploit RPROP2; eauto. i. des. esplits; eauto.
-      eapply nth_error_app_mon. eauto.
-  - (* write failure *)
-    inv STEP; ss. inv ALOCAL_STEP; inv EVENT; ss. esplits; eauto.
-  - (* isb *)
-    inv STEP; ss. inv ALOCAL_STEP; inv EVENT; ss. esplits; ss. all: ss.
-    + i. exploit RPROP1; eauto.
-      apply nth_error_app_inv in GET. des; eauto.
-      apply nth_error_singleton_inv in GET0. des. congr.
-    + i. exploit RPROP2; eauto. i. des. esplits; eauto.
-      eapply nth_error_app_mon. eauto.
-  - (* dmb *)
-    inv STEP; ss. inv ALOCAL_STEP; inv EVENT; ss. esplits; ss. all: ss.
-    + i. exploit RPROP1; eauto.
-      apply nth_error_app_inv in GET. des; eauto.
-      apply nth_error_singleton_inv in GET0. des. congr.
-    + i. exploit RPROP2; eauto. i. des. esplits; eauto.
-      eapply nth_error_app_mon. eauto.
-Admitted.
-
 Inductive co_gen (ws: IdMap.t (list (nat -> option (Loc.t * Time.t)))) (eid1 eid2: eidT): Prop :=
 | co_gen_intro
     w1 wl1 ts1 loc1 w2 wl2 ts2 loc2
@@ -1342,6 +567,442 @@ Definition v_gen (vs: IdMap.t (list (nat -> Time.t))) (eid: eidT): Time.t :=
   end
 .
 
+Inductive sim_th
+          (p:program) (mem:Memory.t) (tid:Id.t)
+          (eu:ExecUnit.t (A:=unit))
+          (aeu:AExecUnit.t)
+          (w: nat -> option (Loc.t * Time.t))
+          (r: nat -> option (Loc.t * Time.t))
+          (cov: nat -> Time.t)
+          (vext: nat -> Time.t): Prop := mk {
+  WPROP1:
+    forall ts loc val
+      (GET: Memory.get_msg ts mem = Some (Msg.mk loc val tid)),
+      ((Promises.lookup ts eu.(ExecUnit.local).(Local.promises) = true /\
+        forall eid, w eid <> Some (loc, ts)) \/
+       (Promises.lookup ts eu.(ExecUnit.local).(Local.promises) = false /\
+        exists eid ex ord,
+          w eid = Some (loc, ts) /\
+          List.nth_error aeu.(AExecUnit.local).(ALocal.labels) eid = Some (Label.write ex ord loc val)));
+  WPROP2:
+    forall eid ex ord loc val
+      (GET: List.nth_error aeu.(AExecUnit.local).(ALocal.labels) eid = Some (Label.write ex ord loc val)),
+    exists ts,
+      w eid = Some (loc, ts) /\
+      Memory.get_msg ts mem = Some (Msg.mk loc val tid);
+  WPROP3:
+    forall eid loc ts (GET: w eid = Some (loc, ts)),
+      Time.lt Time.bot ts /\
+      exists ex ord val,
+        List.nth_error aeu.(AExecUnit.local).(ALocal.labels) eid = Some (Label.write ex ord loc val) /\
+        Memory.get_msg ts mem = Some (Msg.mk loc val tid);
+  WPROP4:
+    forall eid1 loc1 eid2 loc2 ts (W1: w eid1 = Some (loc1, ts)) (W2: w eid2 = Some (loc2, ts)),
+      eid1 = eid2;
+  RPROP1:
+    forall eid ex ord loc val
+      (GET: List.nth_error aeu.(AExecUnit.local).(ALocal.labels) eid = Some (Label.read ex ord loc val)),
+    exists ts tid',
+      r eid = Some (loc, ts) /\
+      __guard__ ((ts = Time.bot /\ val = Val.default) \/
+                 Memory.get_msg ts mem = Some (Msg.mk loc val tid'));
+  RPROP2:
+    forall eid loc ts (GET: r eid = Some (loc, ts)),
+    exists ex ord val tid',
+      List.nth_error aeu.(AExecUnit.local).(ALocal.labels) eid = Some (Label.read ex ord loc val) /\
+      __guard__ ((ts = Time.bot /\ val = Val.default) \/
+                 Memory.get_msg ts mem = Some (Msg.mk loc val tid'));
+  WCV: forall eid ts (W: w eid = Some ts),
+      (exists ex ord loc val,
+          List.nth_error aeu.(AExecUnit.local).(ALocal.labels) eid = Some (Label.write ex ord loc val)) /\
+      cov eid = ts.(snd) /\
+      vext eid = ts.(snd);
+  RCV: forall eid ts (R: r eid = Some ts),
+      (exists ex ord loc val,
+          List.nth_error aeu.(AExecUnit.local).(ALocal.labels) eid = Some (Label.read ex ord loc val)) /\
+      cov eid = ts.(snd);
+  PO: forall iid1 iid2 label1 label2
+     (PO: iid1 < iid2)
+     (LABEL1: List.nth_error aeu.(AExecUnit.local).(ALocal.labels) iid1 = Some label1)
+     (LABEL2: List.nth_error aeu.(AExecUnit.local).(ALocal.labels) iid2 = Some label2)
+     (REL: Execution.label_loc label1 label2),
+      <<PO_LOC_WRITE:
+        Label.is_write label2 ->
+        Time.lt (cov iid1) (cov iid2)>> /\
+      <<PO_LOC_READ:
+        Label.is_read label2 ->
+        Time.le (cov iid1) (cov iid2)>>;
+}.
+
+Lemma sim_trace_sim_th
+      p mem tid
+      tr eu tr'
+      atr aeu atr'
+      wl w wl'
+      rl r rl'
+      covl cov covl'
+      vextl vext vextl'
+      (SIM: sim_trace p mem tid tr atr wl rl covl vextl)
+      (EU: tr = eu :: tr')
+      (AEU: atr = aeu :: atr')
+      (RL: rl = r :: rl')
+      (WL: wl = w :: wl')
+      (COV: covl = cov :: covl')
+      (VEXT: vextl = vext :: vextl'):
+  sim_th p mem tid eu aeu w r cov vext.
+Proof.
+Admitted.
+
+
+(* Lemma sim_trace_vext_cov *)
+(*       p mem tid tr atr wl rl covl vextl *)
+(*       (SIM: sim_trace p mem tid tr atr wl rl covl vextl): *)
+(*   exists aeu atr' w wl' r rl' cov covl' vext vextl', *)
+(*     atr = aeu :: atr' /\ *)
+(*     wl = w :: wl' /\ *)
+(*     rl = r :: rl' /\ *)
+(*     covl = cov :: covl' /\ *)
+(*     vextl = vext :: vextl' /\ *)
+(*     (forall eid ts (W: w eid = Some ts), *)
+(*         (exists ex ord loc val, *)
+(*             List.nth_error aeu.(AExecUnit.local).(ALocal.labels) eid = Some (Label.write ex ord loc val)) /\ *)
+(*         cov eid = ts.(snd) /\ *)
+(*         vext eid = ts.(snd)) /\ *)
+(*     (forall eid ts (R: r eid = Some ts), *)
+(*         (exists ex ord loc val, *)
+(*             List.nth_error aeu.(AExecUnit.local).(ALocal.labels) eid = Some (Label.read ex ord loc val)) /\ *)
+(*         cov eid = ts.(snd)). *)
+(* Proof. *)
+(*   induction SIM; esplits; eauto; i; ss. *)
+(*   - des. simplify. inv EVENT. *)
+(*     + exploit IHSIM4; eauto. i. des. *)
+(*       destruct aeu2. destruct local. *)
+(*       inv ALOCAL_STEP; ss; inv ALOCAL; esplits; eauto. *)
+(*     + des_ifs; eauto. *)
+(*       * exfalso. *)
+(*         rewrite Nat.eqb_eq in Heq. subst. *)
+(*         exploit IHSIM4; eauto. i. des. *)
+(*         unfold ALocal.next_eid in *. *)
+(*         assert (H: List.nth_error (ALocal.labels (AExecUnit.local aeu)) (length (ALocal.labels (AExecUnit.local aeu))) <> None) *)
+(*           by (ii; congr). *)
+(*         rewrite List.nth_error_Some in H. lia. *)
+(*       * exploit IHSIM4; eauto. i. des. *)
+(*         destruct aeu2. destruct local. *)
+(*         inv ALOCAL_STEP; ss; inv ALOCAL; esplits; eauto. *)
+(*         { rewrite List.nth_error_app1; eauto. *)
+(*           eapply List.nth_error_Some. ii. congr. } *)
+(*     + des_ifs; eauto. *)
+(*       * destruct eu1. destruct eu2. *)
+(*         destruct aeu. destruct aeu2. ss. *)
+(*         inv STATE. inv STEP. inv STATE; ss. *)
+(*         rewrite Nat.eqb_eq in Heq. subst. *)
+(*         inv LOCAL; ss. *)
+(*         { inv STEP. ss. splits; eauto. *)
+(*           inv EVENT. inv ALOCAL_STEP; ss. *)
+(*           - esplits. unfold ALocal.next_eid. *)
+(*             rewrite List.nth_error_app2. *)
+(*             rewrite <- Minus.minus_n_n. ss. lia. *)
+(*           - inv EVENT. inv FAILURE. } *)
+(*         { inv STEP. ss. } *)
+(*       * exploit IHSIM4; eauto. i. des. *)
+(*         destruct aeu2. destruct local. *)
+(*         inv ALOCAL_STEP; ss; inv ALOCAL; esplits; eauto. *)
+(*         { rewrite List.nth_error_app1; eauto. *)
+(*           eapply List.nth_error_Some. ii. congr. } *)
+(*       * exploit IHSIM4; eauto. i. des. *)
+(*         destruct aeu2. destruct local. *)
+(*         inv ALOCAL_STEP; ss; inv ALOCAL; esplits; eauto. *)
+(*         { rewrite List.nth_error_app1; eauto. *)
+(*           eapply List.nth_error_Some. ii. congr. } *)
+(*       * exploit IHSIM4; eauto. i. des. *)
+(*         destruct aeu2. destruct local. *)
+(*         inv ALOCAL_STEP; ss; inv ALOCAL; esplits; eauto. *)
+(*         { rewrite List.nth_error_app1; eauto. *)
+(*           eapply List.nth_error_Some. ii. congr. } *)
+(*     + exploit IHSIM4; eauto. i. des. *)
+(*       destruct aeu2. destruct local. *)
+(*       inv ALOCAL_STEP; ss; inv ALOCAL; esplits; eauto. *)
+(*       { rewrite List.nth_error_app1; eauto. *)
+(*         eapply List.nth_error_Some. ii. congr. } *)
+(*   - des. simplify. inv EVENT. *)
+(*     + exploit IHSIM5; eauto. i. des. *)
+(*       destruct aeu2. destruct local. *)
+(*       inv ALOCAL_STEP; ss; inv ALOCAL; esplits; eauto. *)
+(*     + des_ifs; eauto. *)
+(*       * destruct eu1. destruct eu2. *)
+(*         destruct aeu. destruct aeu2. ss. *)
+(*         inv STATE. inv STEP. inv STATE; ss. *)
+(*         rewrite Nat.eqb_eq in Heq. subst. *)
+(*         inv LOCAL; ss. *)
+(*         inv STEP. ss. splits; eauto. *)
+(*         inv EVENT. inv ALOCAL_STEP; ss. *)
+(*         esplits. unfold ALocal.next_eid. *)
+(*         rewrite List.nth_error_app2. *)
+(*         rewrite <- Minus.minus_n_n. ss. lia. *)
+(*       * exploit IHSIM5; eauto. i. des. *)
+(*         destruct aeu2. destruct local. *)
+(*         inv ALOCAL_STEP; ss; inv ALOCAL; esplits; eauto. *)
+(*         { rewrite List.nth_error_app1; eauto. *)
+(*           eapply List.nth_error_Some. ii. congr. } *)
+(*     + des_ifs; eauto. *)
+(*       * exfalso. *)
+(*         rewrite Nat.eqb_eq in Heq. subst. *)
+(*         exploit IHSIM5; eauto. i. des. *)
+(*         unfold ALocal.next_eid in *. *)
+(*         assert (H: List.nth_error (ALocal.labels (AExecUnit.local aeu)) (length (ALocal.labels (AExecUnit.local aeu))) <> None) *)
+(*           by (ii; congr). *)
+(*         rewrite List.nth_error_Some in H. lia. *)
+(*       * exploit IHSIM5; eauto. i. des. *)
+(*         destruct aeu2. destruct local. *)
+(*         inv ALOCAL_STEP; ss; inv ALOCAL; esplits; eauto. *)
+(*         { rewrite List.nth_error_app1; eauto. *)
+(*           eapply List.nth_error_Some. ii. congr. } *)
+(*       * exploit IHSIM5; eauto. i. des. *)
+(*         destruct aeu2. destruct local. *)
+(*         inv ALOCAL_STEP; ss; inv ALOCAL; esplits; eauto. *)
+(*         { rewrite List.nth_error_app1; eauto. *)
+(*           eapply List.nth_error_Some. ii. congr. } *)
+(*       * exploit IHSIM5; eauto. i. des. *)
+(*         destruct aeu2. destruct local. *)
+(*         inv ALOCAL_STEP; ss; inv ALOCAL; esplits; eauto. *)
+(*         { rewrite List.nth_error_app1; eauto. *)
+(*           eapply List.nth_error_Some. ii. congr. } *)
+(*     + exploit IHSIM5; eauto. i. des. *)
+(*       destruct aeu2. destruct local. *)
+(*       inv ALOCAL_STEP; ss; inv ALOCAL; esplits; eauto. *)
+(*       { rewrite List.nth_error_app1; eauto. *)
+(*         eapply List.nth_error_Some. ii. congr. } *)
+(* Qed. *)
+
+(* Lemma sim_trace_cov_po_loc *)
+(*       p mem tid tr atr wl rl cov vext r rl' w wl' eu tr' aeu atr' covf cov' *)
+(*       (SIM: sim_trace p mem tid tr atr wl rl cov vext) *)
+(*       (RL: rl = r :: rl') *)
+(*       (WL: wl = w :: wl') *)
+(*       (EU: tr = eu :: tr') *)
+(*       (AEU: atr = aeu :: atr') *)
+(*       (COV: cov = covf :: cov'): *)
+(*   <<W: forall iid loc ts (W: w iid = Some (loc, ts)), le ts (eu.(ExecUnit.local).(Local.coh) loc)>> /\ *)
+(*   (* TODO: enable it *) *)
+(*   (* (forall iid loc ts (R: r iid = Some (loc, ts), le ts (eu.(ExecUnit.local).(Local.coh) loc)) /\ *) *)
+(*   <<LABEL: forall iid1 iid2 label1 label2 *)
+(*      (PO: iid1 < iid2) *)
+(*      (LABEL1: List.nth_error aeu.(AExecUnit.local).(ALocal.labels) iid1 = Some label1) *)
+(*      (LABEL2: List.nth_error aeu.(AExecUnit.local).(ALocal.labels) iid2 = Some label2) *)
+(*      (REL: Execution.label_loc label1 label2), *)
+(*       <<PO_LOC_WRITE: *)
+(*         Label.is_write label2 -> *)
+(*         Time.lt (covf iid1) (covf iid2)>> /\ *)
+(*       <<PO_LOC_READ: *)
+(*         Label.is_read label2 -> *)
+(*         Time.le (covf iid1) (covf iid2)>>>>. *)
+(* Proof. *)
+(*   revert r rl' w wl' eu tr' aeu atr' covf cov' RL WL EU AEU COV. induction SIM. *)
+(*   { i. simplify. ss. splits; ss. i. destruct iid1; ss. } *)
+(*   i. simplify. *)
+(*   destruct eu1 as [st1 lc1 mem1]. *)
+(*   destruct eu as [st2 lc2 mem2]. *)
+(*   destruct aeu1 as [ast1 alc1]. *)
+(*   destruct aeu as [ast2 alc2]. *)
+(*   ss. exploit IHSIM; eauto. i. des. *)
+(*   inv STEP. inv ALOCAL_STEP; inv EVENT; ss; eauto. *)
+(*   - (* internal *) *)
+(*     admit. *)
+(*   - (* read *) *)
+(*     inv LOCAL; ss. inv ASTATE_STEP; ss. splits; eauto. *)
+(*     { i. etrans; eauto. inv STEP. s. rewrite fun_add_spec. condtac; ss. inversion e. subst. ss. } *)
+(*     i. unfold ALocal.next_eid in *. *)
+(*     apply nth_error_app_inv in LABEL1. *)
+(*     apply nth_error_app_inv in LABEL2. *)
+(*     des. *)
+(*     + repeat condtac; ss. *)
+(*       all: try apply Nat.eqb_eq in X; ss; subst; try lia. *)
+(*       all: try apply Nat.eqb_eq in X0; ss; subst; try lia. *)
+(*       eapply LABEL; eauto. *)
+(*     + lia. *)
+(*     + apply nth_error_singleton_inv in LABEL0. des. subst. *)
+(*       repeat condtac; ss. *)
+(*       all: try apply Nat.eqb_eq in X; ss; subst; try lia. *)
+(*       all: try apply Nat.eqb_neq in X0; ss; try lia. *)
+(*       splits; ss. exploit sim_trace_vext_cov; eauto. i. des. simplify. ss. *)
+      
+      
+(*       admit. *)
+(*     + apply nth_error_singleton_inv in LABEL0. des. subst. *)
+(*       repeat condtac; ss. *)
+(*       all: try apply Nat.eqb_eq in X; ss; try lia. *)
+(*   - (* write *) *)
+(*     inv ASTATE_STEP; ss; eauto. *)
+(*     destruct res1; ss. destruct val; ss. unfold ALocal.next_eid in *. *)
+(*     apply nth_error_app_inv in LABEL1. *)
+(*     apply nth_error_app_inv in LABEL2. *)
+(*     des. *)
+(*     + repeat condtac; ss. *)
+(*       all: try apply Nat.eqb_eq in X; ss; subst; try lia. *)
+(*       all: try apply Nat.eqb_eq in X0; ss; subst; try lia. *)
+(*       eauto. *)
+(*     + apply nth_error_singleton_inv in LABEL3. des. subst. *)
+(*       repeat condtac; ss. *)
+(*       all: try apply Nat.eqb_eq in X; ss; subst; try lia. *)
+(*       all: try apply Nat.eqb_neq in X0; ss; try lia. *)
+(*       admit. *)
+(*     + lia. *)
+(*     + apply nth_error_singleton_inv in LABEL3. des. subst. *)
+(*       repeat condtac; ss. *)
+(*       all: try apply Nat.eqb_eq in X; ss; try lia. *)
+(*   - (* isb *) *)
+(*     destruct res1; ss. destruct val; ss. eauto. *)
+(*   - (* write *) *)
+(*     apply nth_error_app_inv in LABEL1. des; cycle 1. *)
+(*     { apply nth_error_singleton_inv in LABEL0. des. subst. *)
+(*       inv REL. inv X. *)
+(*     } *)
+(*     apply nth_error_app_inv in LABEL2. des; cycle 1. *)
+(*     { apply nth_error_singleton_inv in LtABEL3. des. subst. *)
+(*       inv REL. inv Y. *)
+(*     } *)
+(*     eauto. *)
+(* Admitted. *)
+
+(* Lemma w_property *)
+(*       p mem tid tr atr wl rl covl vextl *)
+(*       (SIM: sim_trace p mem tid tr atr wl rl covl vextl): *)
+(*   exists eu tr' aeu atr' w wl', *)
+(*     tr = eu :: tr' /\ *)
+(*     atr = aeu :: atr' /\ *)
+(*     wl = w :: wl' /\ *)
+(*     <<WPROP1: *)
+(*       forall ts loc val *)
+(*          (GET: Memory.get_msg ts mem = Some (Msg.mk loc val tid)), *)
+(*         ((Promises.lookup ts eu.(ExecUnit.local).(Local.promises) = true /\ *)
+(*           forall eid, w eid <> Some (loc, ts)) \/ *)
+(*          (Promises.lookup ts eu.(ExecUnit.local).(Local.promises) = false /\ *)
+(*           exists eid ex ord, *)
+(*             w eid = Some (loc, ts) /\ *)
+(*             List.nth_error aeu.(AExecUnit.local).(ALocal.labels) eid = Some (Label.write ex ord loc val)))>> /\ *)
+(*     <<WPROP2: *)
+(*       forall eid ex ord loc val *)
+(*         (GET: List.nth_error aeu.(AExecUnit.local).(ALocal.labels) eid = Some (Label.write ex ord loc val)), *)
+(*       exists ts, *)
+(*         w eid = Some (loc, ts) /\ *)
+(*         Memory.get_msg ts mem = Some (Msg.mk loc val tid)>> /\ *)
+(*     <<WPROP3: *)
+(*       forall eid loc ts (GET: w eid = Some (loc, ts)), *)
+(*         Time.lt Time.bot ts /\ *)
+(*       exists ex ord val, *)
+(*         List.nth_error aeu.(AExecUnit.local).(ALocal.labels) eid = Some (Label.write ex ord loc val) /\ *)
+(*         Memory.get_msg ts mem = Some (Msg.mk loc val tid)>> /\ *)
+(*     <<WPROP4: *)
+(*       forall eid1 loc1 eid2 loc2 ts (W1: w eid1 = Some (loc1, ts)) (W2: w eid2 = Some (loc2, ts)), *)
+(*         eid1 = eid2>>. *)
+(* Proof. *)
+(*   induction SIM. *)
+(*   { esplits; ss. *)
+(*     - rewrite IdMap.mapi_spec, STMT in FIND. inv FIND. s. i. *)
+(*       left. splits; ss. admit. (* promises_from_mem *) *)
+(*     - rewrite IdMap.mapi_spec, STMT in FIND. inv FIND. s. i. *)
+(*       destruct eid; ss. *)
+(*   } *)
+(*   des. simplify. *)
+(*   destruct eu as [st1 lc1 mem1]. *)
+(*   destruct eu2 as [st2 lc2 mem2]. *)
+(*   destruct aeu2 as [ast2 alc2]. *)
+(*   ss. inv STEP. inv EVENT; inv LOCAL; inv EVENT; ss. *)
+(*   - (* internal *) *)
+(*     inv LC. s. inv ALOCAL_STEP; inv EVENT; ss. esplits; eauto. *)
+(*   - (* read *) *)
+(*     inv STEP; ss. inv ALOCAL_STEP; inv EVENT; ss. esplits; ss. all: ss. *)
+(*     + i. exploit WPROP1; eauto. i. des; [left|right]; esplits; eauto. *)
+(*       eapply nth_error_app_mon. eauto. *)
+(*     + i. exploit WPROP2; eauto. *)
+(*       apply nth_error_app_inv in GET. des; eauto. *)
+(*       apply nth_error_singleton_inv in GET0. des. congr. *)
+(*     + i. exploit WPROP3; eauto. i. des. esplits; eauto. *)
+(*       eapply nth_error_app_mon. eauto. *)
+(*   - (* write *) *)
+(*     admit. *)
+(*   - (* write failure *) *)
+(*     inv STEP; ss. inv ALOCAL_STEP; inv EVENT; ss. esplits; eauto. *)
+(*   - (* isb *) *)
+(*     inv STEP; ss. inv ALOCAL_STEP; inv EVENT; ss. esplits; ss. all: ss. *)
+(*     + i. exploit WPROP1; eauto. i. des; [left|right]; esplits; eauto. *)
+(*       eapply nth_error_app_mon. eauto. *)
+(*     + i. exploit WPROP2; eauto. *)
+(*       apply nth_error_app_inv in GET. des; eauto. *)
+(*       apply nth_error_singleton_inv in GET0. des. congr. *)
+(*     + i. exploit WPROP3; eauto. i. des. esplits; eauto. *)
+(*       eapply nth_error_app_mon. eauto. *)
+(*   - (* dmb *) *)
+(*     inv STEP; ss. inv ALOCAL_STEP; inv EVENT; ss. esplits; ss. all: ss. *)
+(*     + i. exploit WPROP1; eauto. i. des; [left|right]; esplits; eauto. *)
+(*       eapply nth_error_app_mon. eauto. *)
+(*     + i. exploit WPROP2; eauto. *)
+(*       apply nth_error_app_inv in GET. des; eauto. *)
+(*       apply nth_error_singleton_inv in GET0. des. congr. *)
+(*     + i. exploit WPROP3; eauto. i. des. esplits; eauto. *)
+(*       eapply nth_error_app_mon. eauto. *)
+(* Admitted. *)
+
+(* Lemma r_property *)
+(*       p mem tid tr atr wl rl covl vextl *)
+(*       (SIM: sim_trace p mem tid tr atr wl rl covl vextl): *)
+(*   exists eu tr' aeu atr' r rl', *)
+(*     tr = eu :: tr' /\ *)
+(*     atr = aeu :: atr' /\ *)
+(*     rl = r :: rl' /\ *)
+(*     <<RPROP1: *)
+(*       forall eid ex ord loc val *)
+(*          (GET: List.nth_error aeu.(AExecUnit.local).(ALocal.labels) eid = Some (Label.read ex ord loc val)), *)
+(*       exists ts tid', *)
+(*         r eid = Some (loc, ts) /\ *)
+(*         __guard__ ((ts = Time.bot /\ val = Val.default) \/ *)
+(*          Memory.get_msg ts mem = Some (Msg.mk loc val tid'))>> /\ *)
+(*     <<RPROP2: *)
+(*       forall eid loc ts (GET: r eid = Some (loc, ts)), *)
+(*       exists ex ord val tid', *)
+(*         List.nth_error aeu.(AExecUnit.local).(ALocal.labels) eid = Some (Label.read ex ord loc val) /\ *)
+(*         __guard__ ((ts = Time.bot /\ val = Val.default) \/ *)
+(*          Memory.get_msg ts mem = Some (Msg.mk loc val tid'))>>. *)
+(* Proof. *)
+(*   induction SIM. *)
+(*   { esplits; ss. *)
+(*     rewrite IdMap.mapi_spec, STMT in FIND. inv FIND. s. i. *)
+(*     destruct eid; ss. *)
+(*   } *)
+(*   des. simplify. *)
+(*   destruct eu as [st1 lc1 mem1]. *)
+(*   destruct eu2 as [st2 lc2 mem2]. *)
+(*   destruct aeu2 as [ast2 alc2]. *)
+(*   ss. inv STEP. inv EVENT; inv LOCAL; inv EVENT; ss. *)
+(*   - (* internal *) *)
+(*     inv LC. s. inv ALOCAL_STEP; inv EVENT; ss. esplits; eauto. *)
+(*   - (* read *) *)
+(*     admit. *)
+(*   - (* write *) *)
+(*     inv STEP; ss. inv ALOCAL_STEP; inv EVENT; ss. esplits; ss. all: ss. *)
+(*     + i. exploit RPROP1; eauto. *)
+(*       apply nth_error_app_inv in GET. des; eauto. *)
+(*       apply nth_error_singleton_inv in GET0. des. congr. *)
+(*     + i. exploit RPROP2; eauto. i. des. esplits; eauto. *)
+(*       eapply nth_error_app_mon. eauto. *)
+(*   - (* write failure *) *)
+(*     inv STEP; ss. inv ALOCAL_STEP; inv EVENT; ss. esplits; eauto. *)
+(*   - (* isb *) *)
+(*     inv STEP; ss. inv ALOCAL_STEP; inv EVENT; ss. esplits; ss. all: ss. *)
+(*     + i. exploit RPROP1; eauto. *)
+(*       apply nth_error_app_inv in GET. des; eauto. *)
+(*       apply nth_error_singleton_inv in GET0. des. congr. *)
+(*     + i. exploit RPROP2; eauto. i. des. esplits; eauto. *)
+(*       eapply nth_error_app_mon. eauto. *)
+(*   - (* dmb *) *)
+(*     inv STEP; ss. inv ALOCAL_STEP; inv EVENT; ss. esplits; ss. all: ss. *)
+(*     + i. exploit RPROP1; eauto. *)
+(*       apply nth_error_app_inv in GET. des; eauto. *)
+(*       apply nth_error_singleton_inv in GET0. des. congr. *)
+(*     + i. exploit RPROP2; eauto. i. des. esplits; eauto. *)
+(*       eapply nth_error_app_mon. eauto. *)
+(* Admitted. *)
+
 Lemma sim_traces_co1
       p mem trs atrs rs ws covs vexts ex
       (PRE: Valid.pre_ex p ex)
@@ -1370,15 +1031,16 @@ Proof.
   inv ATR1; inv ATR2; try congr. des.
   rewrite <- H13 in *. rewrite <- H15 in *. ss.
   inv FIND1. inv FIND2.
-  exploit w_property; try exact REL6. i. des.
-  exploit w_property; try exact REL0. i. des.
-  subst. simplify.
-  exploit WPROP2; try exact LABEL; eauto. intro W1. des.
-  exploit WPROP5; try exact LABEL0; eauto. intro W2. des.
+  exploit sim_trace_last; try exact REL6; eauto. i. des. simplify.
+  exploit sim_trace_last; try exact REL0; eauto. i. des. simplify.
+  exploit sim_trace_sim_th; try exact REL6; eauto. intro TH1.
+  exploit sim_trace_sim_th; try exact REL0; eauto. intro TH2.
+  exploit TH1.(WPROP2); try exact LABEL; eauto. intro W1. des.
+  exploit TH2.(WPROP2); try exact LABEL0; eauto. intro W2. des.
   destruct (Id.eq_dec tid1 tid2); subst; simplify.
   - specialize (Nat.lt_trichotomy ts ts0). i. des; subst.
     + right. left. econs; eauto.
-    + exploit WPROP4; [exact W1|exact W2|..]. auto.
+    + exploit TH1.(WPROP4); [exact W1|exact W2|..]. auto.
     + right. right. econs; eauto.
   - specialize (Nat.lt_trichotomy ts ts0). i. des; subst.
     + right. left. econs; eauto.
@@ -1410,10 +1072,12 @@ Proof.
   des. simplify.
   repeat rewrite IdMap.map_spec.
   rewrite <- H13. rewrite <- H15. ss.
-  exploit w_property; try exact REL6. i. des. simplify.
-  exploit w_property; try exact REL0. i. des. simplify.
-  exploit WPROP3; eauto. i. des.
-  exploit WPROP6; eauto. i. des.
+  exploit sim_trace_last; try exact REL6; eauto. i. des. simplify.
+  exploit sim_trace_last; try exact REL0; eauto. i. des. simplify.
+  exploit sim_trace_sim_th; try exact REL6; eauto. intro TH1.
+  exploit sim_trace_sim_th; try exact REL0; eauto. intro TH2.
+  exploit TH1.(WPROP3); eauto. i. des.
+  exploit TH2.(WPROP3); eauto. i. des.
   esplits; eauto.
 Qed.
 
@@ -1444,26 +1108,30 @@ Proof.
   generalize (ATR tid1). intro ATR1. inv ATR1; try congr.
   generalize (SIM tid1). intro SIM1. inv SIM1; try congr.
   des. simplify.
-  exploit r_property; eauto. i. des. simplify.
-  exploit RPROP1; eauto. i. des. unguardH x0. des.
+  exploit sim_trace_last; eauto. i. des. simplify.
+  exploit sim_trace_sim_th; eauto. intro TH.
+  (* exploit r_property; eauto. i. des. simplify. *)
+  exploit TH.(RPROP1); eauto. i. des. unguardH x1. des.
   - left. esplits; subst; eauto.
     ii. inv H. inv H1.
-    destruct x0 as [tid2 eid2]. ss. simplify.
-    rewrite R in x. inv x.
+    destruct x as [tid2 eid2]. ss. simplify.
+    rewrite R in x0. inv x0.
     generalize (SIM tid2). intro SIM1. inv SIM1; try congr.
     simplify.
-    exploit w_property; try exact REL0; eauto. i. des. simplify.
-    exploit WPROP3; eauto. i. des.
+    exploit sim_trace_last; try exact REL0; eauto. i. des. simplify.
+    exploit sim_trace_sim_th; try exact REL0; eauto. intro TH'.
+    exploit TH'.(WPROP3); eauto. i. des.
     unfold Memory.get_msg in x0. ss.
   - right. exploit sim_traces_memory; eauto. i. des.
     generalize (TR tid'). intro TR2. inv TR2; try congr.
     generalize (SIM tid'). intro SIM2. inv SIM2; try congr.
     des. simplify.
-    exploit w_property; try exact REL0; eauto. i. des. simplify.
-    exploit WPROP1; eauto. i. des; ss.
+    exploit sim_trace_last; try exact REL0; eauto. i. des. simplify.
+    exploit sim_trace_sim_th; try exact REL0; eauto. intro TH'.
+    exploit TH'.(WPROP1); eauto. i. des; ss.
     + destruct b. ss. inv NOPROMISE.
-      exploit PROMISES0; eauto. i. rewrite x4 in x1.
-      rewrite Promises.lookup_bot in x1. ss.
+      exploit PROMISES0; eauto. i. rewrite x in x3.
+      rewrite Promises.lookup_bot in x3. ss.
     + generalize (ATR tid'). intro ATR2. inv ATR2; try congr.
       des. simplify. eexists (tid', eid). esplits; ss.
       * rewrite IdMap.map_spec. rewrite <- H8. ss. eauto.
@@ -1510,18 +1178,18 @@ Proof.
   generalize (SIM tid1). intro SIM1. inv SIM1; try congr.
   generalize (SIM tid2). intro SIM2. inv SIM2; try congr.
   simplify.
-  exploit w_property; try exact REL0; eauto. i. des. inv x2.
-  exploit r_property; try exact REL6; eauto. i. des. inv x2.
-  exploit WPROP3; eauto. i. des.
-  exploit RPROP2; eauto. i. des. unguardH x3. des.
-  - rewrite x3 in x1. inv x1.
-  - rewrite x3 in x1. inv x1.
-    generalize (ATR tid1). intro ATR1. inv ATR1; try congr.
-    generalize (ATR tid2). intro ATR2. inv ATR2; try congr.
-    des. simplify. destruct PRE, ex. unfold Execution.label. ss.
-    clear WPROP1 WPROP2 WPROP3 WPROP4 RPROP1 RPROP2.
-    rewrite LABELS. repeat rewrite IdMap.map_spec.
-    rewrite <- H8. rewrite <- H13. ss. esplits; eauto.
+  exploit sim_trace_last; try exact REL0; eauto. i. des. simplify.
+  exploit sim_trace_sim_th; try exact REL0; eauto. intro TH1.
+  exploit sim_trace_last; try exact REL6; eauto. i. des. simplify.
+  exploit sim_trace_sim_th; try exact REL6; eauto. intro TH2.
+  exploit TH1.(WPROP3); eauto. i. des.
+  exploit TH2.(RPROP2); eauto. i. des. unguardH x4. des; subst; ss.
+  rewrite x4 in x2. inv x2.
+  generalize (ATR tid1). intro ATR1. inv ATR1; try congr.
+  generalize (ATR tid2). intro ATR2. inv ATR2; try congr.
+  des. simplify. destruct PRE, ex. unfold Execution.label. ss.
+  rewrite LABELS. repeat rewrite IdMap.map_spec.
+  rewrite <- H8. rewrite <- H13. ss. esplits; eauto.
 Qed.
 
 Lemma sim_traces_rf_wf
@@ -1534,136 +1202,19 @@ Proof.
   simplify. rewrite R in R0. inv R0.
   destruct (Id.eq_dec tid1 tid2); subst; simplify.
   - specialize (SIM tid2). inv SIM; try congr.
-    exploit w_property; eauto. i. des. simplify.
-    exploit WPROP4; [exact W|exact W0|..]. i. subst. refl.
+    exploit sim_trace_last; eauto. i. des. simplify.
+    exploit sim_trace_sim_th; eauto. intro TH.
+    exploit TH.(WPROP4); [exact W|exact W0|..]. i. subst. refl.
   - generalize (SIM tid1). intro SIM1. inv SIM1; try congr.
     generalize (SIM tid2). intro SIM2. inv SIM2; try congr.
-    exploit w_property; try exact REL6; eauto. i. des.
-    exploit w_property; try exact REL0; eauto. i. des.
+    exploit sim_trace_last; try exact REL6; eauto. i. des. simplify.
+    exploit sim_trace_sim_th; try exact REL6; eauto. intro TH1.
+    exploit sim_trace_last; try exact REL0; eauto. i. des. simplify.
+    exploit sim_trace_sim_th; try exact REL0; eauto. intro TH2.
     simplify.
-    exploit WPROP3; eauto. i. des.
-    exploit WPROP6; eauto. i. des.
+    exploit TH1.(WPROP3); eauto. i. des.
+    exploit TH2.(WPROP3); eauto. i. des.
     congr.
-Qed.
-
-Lemma sim_trace_vext_cov
-      p mem tid tr atr wl rl covl vextl
-      (SIM: sim_trace p mem tid tr atr wl rl covl vextl):
-  exists aeu atr' w wl' r rl' cov covl' vext vextl',
-    atr = aeu :: atr' /\
-    wl = w :: wl' /\
-    rl = r :: rl' /\
-    covl = cov :: covl' /\
-    vextl = vext :: vextl' /\
-    (forall eid ts (W: w eid = Some ts),
-        (exists ex ord loc val,
-            List.nth_error aeu.(AExecUnit.local).(ALocal.labels) eid = Some (Label.write ex ord loc val)) /\
-        cov eid = ts.(snd) /\
-        vext eid = ts.(snd)) /\
-    (forall eid ts (R: r eid = Some ts),
-        (exists ex ord loc val,
-            List.nth_error aeu.(AExecUnit.local).(ALocal.labels) eid = Some (Label.read ex ord loc val)) /\
-        cov eid = ts.(snd)).
-Proof.
-  induction SIM; esplits; eauto; i; ss.
-  - des. simplify. inv EVENT.
-    + exploit IHSIM4; eauto. i. des.
-      destruct aeu2. destruct local.
-      inv ALOCAL_STEP; ss; inv ALOCAL; esplits; eauto.
-    + des_ifs; eauto.
-      * exfalso.
-        rewrite Nat.eqb_eq in Heq. subst.
-        exploit IHSIM4; eauto. i. des.
-        unfold ALocal.next_eid in *.
-        assert (H: List.nth_error (ALocal.labels (AExecUnit.local aeu)) (length (ALocal.labels (AExecUnit.local aeu))) <> None)
-          by (ii; congr).
-        rewrite List.nth_error_Some in H. lia.
-      * exploit IHSIM4; eauto. i. des.
-        destruct aeu2. destruct local.
-        inv ALOCAL_STEP; ss; inv ALOCAL; esplits; eauto.
-        { rewrite List.nth_error_app1; eauto.
-          eapply List.nth_error_Some. ii. congr. }
-    + des_ifs; eauto.
-      * destruct eu1. destruct eu2.
-        destruct aeu. destruct aeu2. ss.
-        inv STATE. inv STEP. inv STATE; ss.
-        rewrite Nat.eqb_eq in Heq. subst.
-        inv LOCAL; ss.
-        { inv STEP. ss. splits; eauto.
-          inv EVENT. inv ALOCAL_STEP; ss.
-          - esplits. unfold ALocal.next_eid.
-            rewrite List.nth_error_app2.
-            rewrite <- Minus.minus_n_n. ss. lia.
-          - inv EVENT. inv FAILURE. }
-        { inv STEP. ss. }
-      * exploit IHSIM4; eauto. i. des.
-        destruct aeu2. destruct local.
-        inv ALOCAL_STEP; ss; inv ALOCAL; esplits; eauto.
-        { rewrite List.nth_error_app1; eauto.
-          eapply List.nth_error_Some. ii. congr. }
-      * exploit IHSIM4; eauto. i. des.
-        destruct aeu2. destruct local.
-        inv ALOCAL_STEP; ss; inv ALOCAL; esplits; eauto.
-        { rewrite List.nth_error_app1; eauto.
-          eapply List.nth_error_Some. ii. congr. }
-      * exploit IHSIM4; eauto. i. des.
-        destruct aeu2. destruct local.
-        inv ALOCAL_STEP; ss; inv ALOCAL; esplits; eauto.
-        { rewrite List.nth_error_app1; eauto.
-          eapply List.nth_error_Some. ii. congr. }
-    + exploit IHSIM4; eauto. i. des.
-      destruct aeu2. destruct local.
-      inv ALOCAL_STEP; ss; inv ALOCAL; esplits; eauto.
-      { rewrite List.nth_error_app1; eauto.
-        eapply List.nth_error_Some. ii. congr. }
-  - des. simplify. inv EVENT.
-    + exploit IHSIM5; eauto. i. des.
-      destruct aeu2. destruct local.
-      inv ALOCAL_STEP; ss; inv ALOCAL; esplits; eauto.
-    + des_ifs; eauto.
-      * destruct eu1. destruct eu2.
-        destruct aeu. destruct aeu2. ss.
-        inv STATE. inv STEP. inv STATE; ss.
-        rewrite Nat.eqb_eq in Heq. subst.
-        inv LOCAL; ss.
-        inv STEP. ss. splits; eauto.
-        inv EVENT. inv ALOCAL_STEP; ss.
-        esplits. unfold ALocal.next_eid.
-        rewrite List.nth_error_app2.
-        rewrite <- Minus.minus_n_n. ss. lia.
-      * exploit IHSIM5; eauto. i. des.
-        destruct aeu2. destruct local.
-        inv ALOCAL_STEP; ss; inv ALOCAL; esplits; eauto.
-        { rewrite List.nth_error_app1; eauto.
-          eapply List.nth_error_Some. ii. congr. }
-    + des_ifs; eauto.
-      * exfalso.
-        rewrite Nat.eqb_eq in Heq. subst.
-        exploit IHSIM5; eauto. i. des.
-        unfold ALocal.next_eid in *.
-        assert (H: List.nth_error (ALocal.labels (AExecUnit.local aeu)) (length (ALocal.labels (AExecUnit.local aeu))) <> None)
-          by (ii; congr).
-        rewrite List.nth_error_Some in H. lia.
-      * exploit IHSIM5; eauto. i. des.
-        destruct aeu2. destruct local.
-        inv ALOCAL_STEP; ss; inv ALOCAL; esplits; eauto.
-        { rewrite List.nth_error_app1; eauto.
-          eapply List.nth_error_Some. ii. congr. }
-      * exploit IHSIM5; eauto. i. des.
-        destruct aeu2. destruct local.
-        inv ALOCAL_STEP; ss; inv ALOCAL; esplits; eauto.
-        { rewrite List.nth_error_app1; eauto.
-          eapply List.nth_error_Some. ii. congr. }
-      * exploit IHSIM5; eauto. i. des.
-        destruct aeu2. destruct local.
-        inv ALOCAL_STEP; ss; inv ALOCAL; esplits; eauto.
-        { rewrite List.nth_error_app1; eauto.
-          eapply List.nth_error_Some. ii. congr. }
-    + exploit IHSIM5; eauto. i. des.
-      destruct aeu2. destruct local.
-      inv ALOCAL_STEP; ss; inv ALOCAL; esplits; eauto.
-      { rewrite List.nth_error_app1; eauto.
-        eapply List.nth_error_Some. ii. congr. }
 Qed.
 
 Lemma sim_traces_cov_co
@@ -1680,12 +1231,14 @@ Proof.
   destruct eid1 as [tid1 eid1], eid2 as [tid2 eid2]. ss.
   generalize (SIM tid1). intro SIM1. inv SIM1; try congr.
   generalize (SIM tid2). intro SIM2. inv SIM2; try congr. simplify.
-  exploit sim_trace_vext_cov; try exact REL6. i. des.
-  exploit sim_trace_vext_cov; try exact REL0. i. des. simplify.
-  exploit x5; eauto. i. des.
-  exploit x12; eauto. i. des.
+  exploit sim_trace_last; try exact REL6; eauto. i. des. simplify.
+  exploit sim_trace_sim_th; try exact REL6; eauto. intro TH1.
+  exploit sim_trace_last; try exact REL0; eauto. i. des. simplify.
+  exploit sim_trace_sim_th; try exact REL0; eauto. intro TH2.
+  exploit TH1.(WCV); eauto. i. des.
+  exploit TH2.(WCV); eauto. i. des.
   unfold v_gen. ss. rewrite <- H4. rewrite <- H10.
-  rewrite x0. rewrite x3. auto.
+  rewrite x1, x4. auto.
 Qed.
 
 Lemma sim_traces_cov_rf
@@ -1702,12 +1255,14 @@ Proof.
   destruct eid1 as [tid1 eid1], eid2 as [tid2 eid2]. ss.
   generalize (SIM tid1). intro SIM1. inv SIM1; try congr.
   generalize (SIM tid2). intro SIM2. inv SIM2; try congr. simplify.
-  exploit sim_trace_vext_cov; try exact REL6. i. des.
-  exploit sim_trace_vext_cov; try exact REL0. i. des. simplify.
-  exploit x5; eauto. i. des.
-  exploit x13; eauto. i. des.
+  exploit sim_trace_last; try exact REL6; eauto. i. des. simplify.
+  exploit sim_trace_sim_th; try exact REL6; eauto. intro TH1.
+  exploit sim_trace_last; try exact REL0; eauto. i. des. simplify.
+  exploit sim_trace_sim_th; try exact REL0; eauto. intro TH2.
+  exploit TH1.(WCV); eauto. i. des.
+  exploit TH2.(RCV); eauto. i. des.
   unfold v_gen. ss. rewrite <- H4. rewrite <- H10.
-  rewrite x0. rewrite x3. refl.
+  rewrite x1, x4. refl.
 Qed.
 
 Lemma sim_traces_cov_fr
@@ -1744,111 +1299,22 @@ Proof.
       destruct (IdMap.find tid2 aeus) eqn:FIND2; ss.
       generalize (ATR tid2). intro ATR2. inv ATR2; try congr. des. simplify.
       generalize (SIM tid2). intro SIM2. inv SIM2; try congr. simplify.
-      exploit w_property; try exact REL6. i. des. simplify.
-      exploit WPROP2; eauto. i. des.
-      exploit WPROP3; eauto. i. des.
-      clear ex2 ord1 val0 x2 x3.
+      exploit sim_trace_last; try exact REL6; eauto. i. des. simplify.
+      exploit sim_trace_sim_th; try exact REL6; eauto. intro TH1.
+      exploit TH1.(WPROP2); eauto. i. des.
+      exploit TH1.(WPROP3); eauto. i. des.
+      clear ex2 ord1 val0 x3 x4.
       generalize (SIM tid1). intro SIM1. inv SIM1; try congr. simplify.
-      exploit sim_trace_vext_cov; try exact REL6. i. des.
-      exploit sim_trace_vext_cov; try exact REL0. i. des. simplify.
-      exploit x7; eauto. i. des.
-      exploit x15; eauto. i. des.
+      exploit sim_trace_last; try exact REL0; eauto. i. des. simplify.
+      exploit sim_trace_sim_th; try exact REL0; eauto. intro TH2.
+      exploit TH1.(WCV); eauto. i. des.
+      exploit TH2.(RCV); eauto. i. des.
       unfold v_gen. ss. rewrite <- H12. rewrite <- H7.
-      rewrite x6. rewrite x3. auto.
+      rewrite x7, x4. auto.
     + exfalso.
       rewrite RF in *. eapply H3. unfold codom_rel.
       eexists. eauto.
 Qed.
-
-Lemma sim_traces_cov_po_loc_aux
-      p mem tid tr atr wl rl cov vext r rl' w wl' eu tr' aeu atr' covf cov'
-      (SIM: sim_trace p mem tid tr atr wl rl cov vext)
-      (RL: rl = r :: rl')
-      (WL: wl = w :: wl')
-      (EU: tr = eu :: tr')
-      (AEU: atr = aeu :: atr')
-      (COV: cov = covf :: cov'):
-  <<W: forall iid loc ts (W: w iid = Some (loc, ts)), le ts (eu.(ExecUnit.local).(Local.coh) loc)>> /\
-  (* TODO: enable it *)
-  (* (forall iid loc ts (R: r iid = Some (loc, ts), le ts (eu.(ExecUnit.local).(Local.coh) loc)) /\ *)
-  <<LABEL: forall iid1 iid2 label1 label2
-     (PO: iid1 < iid2)
-     (LABEL1: List.nth_error aeu.(AExecUnit.local).(ALocal.labels) iid1 = Some label1)
-     (LABEL2: List.nth_error aeu.(AExecUnit.local).(ALocal.labels) iid2 = Some label2)
-     (REL: Execution.label_loc label1 label2),
-      <<PO_LOC_WRITE:
-        Label.is_write label2 ->
-        Time.lt (covf iid1) (covf iid2)>> /\
-      <<PO_LOC_READ:
-        Label.is_read label2 ->
-        Time.le (covf iid1) (covf iid2)>>>>.
-Proof.
-  revert r rl' w wl' eu tr' aeu atr' covf cov' RL WL EU AEU COV. induction SIM.
-  { i. simplify. ss. splits; ss. i. destruct iid1; ss. }
-  i. simplify.
-  destruct eu1 as [st1 lc1 mem1].
-  destruct eu as [st2 lc2 mem2].
-  destruct aeu1 as [ast1 alc1].
-  destruct aeu as [ast2 alc2].
-  ss. exploit IHSIM; eauto. i. des.
-  inv STEP. inv ALOCAL_STEP; inv EVENT; ss; eauto.
-  - (* internal *)
-    admit.
-  - (* read *)
-    inv LOCAL; ss. inv ASTATE_STEP; ss. splits; eauto.
-    { i. etrans; eauto. inv STEP. s. rewrite fun_add_spec. condtac; ss. inversion e. subst. ss. }
-    i. unfold ALocal.next_eid in *.
-    apply nth_error_app_inv in LABEL1.
-    apply nth_error_app_inv in LABEL2.
-    des.
-    + repeat condtac; ss.
-      all: try apply Nat.eqb_eq in X; ss; subst; try lia.
-      all: try apply Nat.eqb_eq in X0; ss; subst; try lia.
-      eapply LABEL; eauto.
-    + lia.
-    + apply nth_error_singleton_inv in LABEL0. des. subst.
-      repeat condtac; ss.
-      all: try apply Nat.eqb_eq in X; ss; subst; try lia.
-      all: try apply Nat.eqb_neq in X0; ss; try lia.
-      splits; ss. exploit sim_trace_vext_cov; eauto. i. des. simplify. ss.
-      
-      
-      admit.
-    + apply nth_error_singleton_inv in LABEL0. des. subst.
-      repeat condtac; ss.
-      all: try apply Nat.eqb_eq in X; ss; try lia.
-  - (* write *)
-    inv ASTATE_STEP; ss; eauto.
-    destruct res1; ss. destruct val; ss. unfold ALocal.next_eid in *.
-    apply nth_error_app_inv in LABEL1.
-    apply nth_error_app_inv in LABEL2.
-    des.
-    + repeat condtac; ss.
-      all: try apply Nat.eqb_eq in X; ss; subst; try lia.
-      all: try apply Nat.eqb_eq in X0; ss; subst; try lia.
-      eauto.
-    + apply nth_error_singleton_inv in LABEL3. des. subst.
-      repeat condtac; ss.
-      all: try apply Nat.eqb_eq in X; ss; subst; try lia.
-      all: try apply Nat.eqb_neq in X0; ss; try lia.
-      admit.
-    + lia.
-    + apply nth_error_singleton_inv in LABEL3. des. subst.
-      repeat condtac; ss.
-      all: try apply Nat.eqb_eq in X; ss; try lia.
-  - (* isb *)
-    destruct res1; ss. destruct val; ss. eauto.
-  - (* write *)
-    apply nth_error_app_inv in LABEL1. des; cycle 1.
-    { apply nth_error_singleton_inv in LABEL0. des. subst.
-      inv REL. inv X.
-    }
-    apply nth_error_app_inv in LABEL2. des; cycle 1.
-    { apply nth_error_singleton_inv in LtABEL3. des. subst.
-      inv REL. inv Y.
-    }
-    eauto.
-Admitted.
 
 Lemma sim_traces_cov_po_loc
       p mem trs atrs ws rs covs vexts
@@ -1871,7 +1337,8 @@ Proof.
   generalize (ATR tid2). intro X. inv X; ss; rewrite <- H in *; ss.
   des. subst. generalize (SIM tid2). i. inv H1; simplify.
   exploit sim_trace_last; eauto. i. des. subst. simplify.
-  exploit sim_traces_cov_po_loc_aux; eauto. i. des.
+  exploit sim_trace_sim_th; eauto. intro TH.
+  exploit TH.(PO); eauto. i. des.
   unfold v_gen. s. rewrite <- H7. splits; i.
   - inv H1. unfold Execution.label in *. ss.
     rewrite PRE.(Valid.LABELS), IdMap.map_spec, <- H in *. inv EID.
@@ -1895,80 +1362,14 @@ Proof.
   destruct eid1 as [tid1 eid1], eid2 as [tid2 eid2]. ss.
   generalize (SIM tid1). intro SIM1. inv SIM1; try congr.
   generalize (SIM tid2). intro SIM2. inv SIM2; try congr. simplify.
-  exploit sim_trace_vext_cov; try exact REL6. i. des.
-  exploit sim_trace_vext_cov; try exact REL0. i. des. simplify.
-  exploit x5; eauto. i. des.
-  exploit x12; eauto. i. des.
+  exploit sim_trace_last; try exact REL6; eauto. i. des. simplify.
+  exploit sim_trace_sim_th; try exact REL6; eauto. intro TH1.
+  exploit sim_trace_last; try exact REL0; eauto. i. des. simplify.
+  exploit sim_trace_sim_th; try exact REL0; eauto. intro TH2.
+  exploit TH1.(WCV); eauto. i. des.
+  exploit TH2.(WCV); eauto. i. des.
   unfold v_gen. ss. rewrite <- H5. rewrite <- H11.
-  rewrite x1. rewrite x4. auto.
-Qed.
-
-Definition lastn A (n: nat) (l: list A) :=
-  List.rev (List.firstn n (List.rev l)).
-
-Lemma lastn_snoc A n (l:list A) x:
-  lastn (S n) (l ++ [x]) = (lastn n l) ++ [x].
-Proof.
-  revert n. induction l using List.rev_ind; ss.
-  unfold lastn. s. rewrite List.rev_app_distr. ss.
-Qed.
-
-Lemma lastn_cons A n a (l:list A)
-      (N: n <= length l):
-  lastn n (a::l) = lastn n l.
-Proof.
-  revert n N. induction l using List.rev_ind; ss.
-  { i. destruct n; ss. unfold lastn. s. destruct n; lia. }
-  i. destruct n; ss. rewrite List.app_comm_cons, ? lastn_snoc. f_equal.
-  eapply IHl. rewrite List.app_length in N. ss. lia.
-Qed.
-
-Lemma lastn_one A
-      (l: list A)
-      (LENGTH: List.length l >= 1):
-  exists a, lastn 1 l = [a].
-Proof.
-  destruct l using List.rev_ind; ss; [lia|]. rewrite lastn_snoc. s. eauto.
-Qed.
-
-Lemma lastn_all A n (l: list A)
-      (N: n >= length l):
-  lastn n l = l.
-Proof.
-  revert n N. induction l using List.rev_ind; ss.
-  { destruct n; ss. }
-  i. rewrite List.app_length in N. ss. destruct n; [lia|].
-  rewrite lastn_snoc, IHl; ss. lia.
-Qed.
-
-Lemma lastn_length A n (l: list A):
-  length (lastn n l) = min n (length l).
-Proof.
-  revert n. induction l using List.rev_ind; ss.
-  { destruct n; ss. }
-  i. destruct n; ss. rewrite lastn_snoc, ? List.app_length, IHl. s.
-  rewrite (Nat.add_comm (length l)). s. lia.
-Qed.
-
-Lemma lastn_S A n (l: list A)
-      (LENGTH: List.length l > 0):
-  exists a l', lastn (S n) l = a :: l'.
-Proof.
-  generalize (lastn_length (S n) l). i.
-  destruct (lastn (S n) l) eqn:LASTN; eauto.
-  destruct l; ss. lia.
-Qed.
-
-Lemma lastn_S1 A
-      (l: list A) n a l'
-      (N: n < List.length l)
-      (LASTN: lastn (S n) l = a :: l'):
-  lastn n l = l'.
-Proof.
-  rewrite <- List.rev_length in N. apply List.nth_error_Some in N.
-  destruct (List.nth_error (List.rev l) n) eqn:NTH; ss.
-  revert LASTN. unfold lastn. erewrite List_firstn_S; eauto.
-  rewrite List.rev_app_distr. s. i. inv LASTN. ss.
+  rewrite x5, x2. auto.
 Qed.
 
 Lemma sim_trace_lastn
