src/axiomatic/CommonAxiomatic.v
@@ -1,0 +1,587 @@
+Require Import Relations.
+Require Import Permutation.
+Require Import NArith.
+Require Import PArith.
+Require Import ZArith.
+Require Import Lia.
+Require Import FMapPositive.
+Require Import FSetPositive.
+Require Import EquivDec.
+Require Import sflib.
+Require Import paco.
+Require Import HahnRelationsBasic.
+
+Require Import PromisingArch.lib.Basic.
+Require Import PromisingArch.lib.HahnRelationsMore.
+Require Import PromisingArch.lib.Order.
+Require Import PromisingArch.lib.Time.
+Require Import PromisingArch.lib.Lang.
+Require Import PromisingArch.promising.Promising.
+Require Import PromisingArch.promising.StateExecFacts.
+Require Import PromisingArch.axiomatic.Axiomatic.
+
+Set Implicit Arguments.
+
+
+Inductive inverse A (rel:relation A) (codom:A -> Prop) (a:A): Prop :=
+| inverse_intro
+    a'
+    (REL: rel a a')
+    (CODOM: codom a')
+.
+Hint Constructors inverse.
+
+Lemma inverse_mon A (r1 r2:relation A)
+      (REL: r1 ⊆ r2):
+  inverse r1 <2= inverse r2.
+Proof.
+  i. inv PR. econs; eauto.
+Qed.
+
+Lemma inverse_union A (r1 r2:relation A) s:
+  inverse (r1 ∪ r2) s = inverse r1 s \1/ inverse r2 s.
+Proof.
+  funext. i. propext. econs; i.
+  - inv H. inv REL; eauto.
+  - des; inv H; econs; eauto.
+    + left. ss.
+    + right. ss.
+Qed.
+
+Lemma inverse_step
+      r tid n:
+  inverse (r ⨾ Execution.po_adj) (eq (tid, S n)) = inverse r (eq (tid, n)).
+Proof.
+  funext. i. propext. econs; i.
+  - inv H. inv REL. des. inv H0. destruct x, x0. ss. inv N. econs; eauto.
+  - inv H. econs; eauto. econs; eauto.
+Qed.
+
+Definition sim_local_coh ex loc :=
+  ⦗ex.(Execution.label_is) (Label.is_writing loc)⦘ ⨾
+  ex.(Execution.rfe)^? ⨾
+  Execution.po.
+
+Lemma sim_local_coh_step ex loc:
+  sim_local_coh ex loc =
+  (sim_local_coh ex loc ∪
+   ⦗ex.(Execution.label_is) (Label.is_writing loc)⦘ ⨾ ex.(Execution.rfe)^?) ⨾
+  Execution.po_adj.
+Proof.
+  unfold sim_local_coh. rewrite Execution.po_po_adj at 1.
+  rewrite (clos_refl_union Execution.po), union_seq, eq_seq.
+  rewrite ? seq_union, ? union_seq, ? seq_assoc.
+  refl.
+Qed.
+
+Lemma sim_local_coh_spec
+      p ex loc eid1 eid2
+      (EX: Valid.ex p ex)
+      (EID2: Execution.label_is ex (Label.is_accessing loc) eid2)
+      (COH: sim_local_coh ex loc eid1 eid2):
+  <<INTERNAL: ex.(Execution.internal)⁺ eid1 eid2>> /\
+  <<LABEL: Execution.label_is ex (Label.is_writing loc) eid1>>.
+Proof.
+  inv COH. des. inv H. inv H0. des. inv EID2. inv H2. destruct l0; ss. inv H.
+  - esplits.
+    + econs. left. left. left. econs; eauto.
+    + destruct (equiv_dec loc0 loc); ss. inv e. econs; eauto. apply Label.write_is_writing.
+  - inv H1. splits.
+    + econs 2; [econs|].
+      { right. eauto. }
+      exploit EX.(Valid.RF2); eauto. i. des.
+      rewrite EID0 in WRITE. inv WRITE.
+      econs. left. left. left. econs; eauto.
+    + destruct (equiv_dec loc0 loc); ss. inv e. econs; eauto. apply Label.write_is_writing.
+Qed.
+
+Definition sim_local_vrp ex :=
+  (⦗ex.(Execution.label_is) Label.is_read⦘ ⨾
+   Execution.po ⨾
+   ⦗ex.(Execution.label_is) (Label.is_barrier_c Barrier.is_dmb_rr)⦘ ⨾
+   Execution.po) ∪
+
+  (⦗ex.(Execution.label_is) Label.is_write⦘ ⨾
+   Execution.po ⨾
+   ⦗ex.(Execution.label_is) (Label.is_barrier_c Barrier.is_dmb_wr)⦘ ⨾
+   Execution.po) ∪
+
+  ((ex.(Execution.ctrl) ∪ (ex.(Execution.addr) ⨾ Execution.po)) ⨾
+   ⦗ex.(Execution.label_is) (eq (Label.barrier Barrier.isb))⦘ ⨾
+   Execution.po) ∪
+
+  (⦗ex.(Execution.label_is) (Label.is_acquire_pc)⦘ ⨾
+   Execution.po).
+
+Lemma sim_local_vrp_step ex:
+  sim_local_vrp ex =
+  (sim_local_vrp ex ∪
+   ((⦗ex.(Execution.label_is) Label.is_read⦘ ⨾
+     Execution.po ⨾
+     ⦗ex.(Execution.label_is) (Label.is_barrier_c Barrier.is_dmb_rr)⦘) ∪
+
+   (⦗ex.(Execution.label_is) Label.is_write⦘ ⨾
+     Execution.po ⨾
+     ⦗ex.(Execution.label_is) (Label.is_barrier_c Barrier.is_dmb_wr)⦘) ∪
+
+    ((ex.(Execution.ctrl) ∪ (ex.(Execution.addr) ⨾ Execution.po)) ⨾
+     ⦗ex.(Execution.label_is) (eq (Label.barrier Barrier.isb))⦘) ∪
+
+    (⦗ex.(Execution.label_is) (Label.is_acquire_pc)⦘))) ⨾
+  Execution.po_adj.
+Proof.
+  unfold sim_local_vrp. rewrite ? (union_seq' Execution.po_adj), ? seq_assoc, ? union_assoc.
+  rewrite Execution.po_po_adj at 2 4 6 7.
+  rewrite (clos_refl_union Execution.po), union_seq, eq_seq.
+  rewrite ? (seq_union' (Execution.po ⨾ Execution.po_adj) Execution.po_adj), ? seq_assoc, ? union_assoc.
+  funext. i. funext. i. propext. econs; i.
+  - repeat match goal with
+           | [H: (_ ∪ _) _ _ |- _] => inv H
+           end;
+      eauto 10 using union_l, union_r.
+  - repeat match goal with
+           | [H: (_ ∪ _) _ _ |- _] => inv H
+           end;
+      eauto 10 using union_l, union_r.
+Qed.
+
+Lemma sim_local_vrp_spec
+      p ex eid1 eid2
+      (EX: Valid.ex p ex)
+      (EID2: Execution.label_is ex Label.is_read eid2)
+      (VRP: sim_local_vrp ex eid1 eid2):
+  <<OB: ex.(Execution.ob) eid1 eid2>>.
+Proof.
+  inv EID2. destruct l; inv LABEL. unfold sim_local_vrp in VRP.
+  repeat match goal with
+         | [H: (_ ∪ _) _ _ |- _] => inv H
+         end.
+  - right. left. left. left. left. left. left. left.
+    inv H. des. econs. splits; eauto.
+    rewrite ? seq_assoc. econs. splits; [|by econs; eauto].
+    rewrite <- ? seq_assoc. ss.
+  - right. left. left. left. left. left. right.
+    inv H. des. econs. splits; eauto.
+    rewrite ? seq_assoc. econs. splits; [|by econs; eauto].
+    rewrite <- ? seq_assoc. ss.
+  - left. left. right. right.
+    inv H0. des. econs. splits; eauto.
+    right. rewrite seq_assoc. econs. splits; eauto. econs; ss. econs; eauto.
+  - right. left. left. right.
+    inv H. des. econs. splits; eauto.
+Qed.
+
+Definition sim_local_vwp ex :=
+  (⦗ex.(Execution.label_is) Label.is_read⦘ ⨾
+   Execution.po ⨾
+   ⦗ex.(Execution.label_is) (Label.is_barrier_c Barrier.is_dmb_rw)⦘ ⨾
+   Execution.po) ∪
+
+  (⦗ex.(Execution.label_is) Label.is_write⦘ ⨾
+   Execution.po ⨾
+   ⦗ex.(Execution.label_is) (Label.is_barrier_c Barrier.is_dmb_ww)⦘ ⨾
+   Execution.po) ∪
+
+  (⦗ex.(Execution.label_is) (Label.is_acquire_pc)⦘ ⨾
+   Execution.po).
+
+Lemma sim_local_vwp_step ex:
+  sim_local_vwp ex =
+  (sim_local_vwp ex ∪
+   ((⦗ex.(Execution.label_is) Label.is_read⦘ ⨾
+     Execution.po ⨾
+     ⦗ex.(Execution.label_is) (Label.is_barrier_c Barrier.is_dmb_rw)⦘) ∪
+
+   (⦗ex.(Execution.label_is) Label.is_write⦘ ⨾
+     Execution.po ⨾
+     ⦗ex.(Execution.label_is) (Label.is_barrier_c Barrier.is_dmb_ww)⦘) ∪
+
+    (⦗ex.(Execution.label_is) (Label.is_acquire_pc)⦘))) ⨾
+  Execution.po_adj.
+Proof.
+  unfold sim_local_vwp. rewrite ? (union_seq' Execution.po_adj), ? seq_assoc, ? union_assoc.
+  rewrite Execution.po_po_adj at 2 4 5.
+  rewrite (clos_refl_union Execution.po), union_seq, eq_seq.
+  rewrite ? (seq_union' (Execution.po ⨾ Execution.po_adj) Execution.po_adj), ? seq_assoc, ? union_assoc.
+  funext. i. funext. i. propext. econs; i.
+  - repeat match goal with
+           | [H: (_ ∪ _) _ _ |- _] => inv H
+           end;
+      eauto 10 using union_l, union_r.
+  - repeat match goal with
+           | [H: (_ ∪ _) _ _ |- _] => inv H
+           end;
+      eauto 10 using union_l, union_r.
+Qed.
+
+Lemma sim_local_vwp_spec
+      p ex eid1 eid2
+      (EX: Valid.ex p ex)
+      (EID2: Execution.label_is ex Label.is_write eid2)
+      (VWP: sim_local_vwp ex eid1 eid2):
+  <<OB: ex.(Execution.ob) eid1 eid2>>.
+Proof.
+  inv EID2. destruct l; inv LABEL. unfold sim_local_vwp in VWP.
+  repeat match goal with
+         | [H: (_ ∪ _) _ _ |- _] => inv H
+         end.
+  - right. left. left. left. left. left. left. right.
+    inv H0. des. econs. splits; eauto.
+    rewrite ? seq_assoc. econs. splits; [|by econs; eauto].
+    rewrite <- ? seq_assoc. ss.
+  - right. left. left. left. left. right.
+    inv H0. des. econs. splits; eauto.
+    rewrite ? seq_assoc. econs. splits; [|by econs; eauto].
+    rewrite <- ? seq_assoc. ss.
+  - right. left. left. right.
+    inv H. des. econs. splits; eauto.
+Qed.
+
+Definition sim_local_vrm ex :=
+  ⦗ex.(Execution.label_is) (Label.is_read)⦘ ⨾ Execution.po.
+
+Lemma sim_local_vrm_step ex:
+  sim_local_vrm ex =
+  (sim_local_vrm ex ∪ ⦗ex.(Execution.label_is) (Label.is_read)⦘) ⨾
+  Execution.po_adj.
+Proof.
+  unfold sim_local_vrm. rewrite ? (union_seq' Execution.po_adj), ? seq_assoc, ? union_assoc.
+  rewrite Execution.po_po_adj at 1.
+  rewrite (clos_refl_union Execution.po), union_seq, eq_seq.
+  rewrite ? (seq_union' (Execution.po ⨾ Execution.po_adj) Execution.po_adj), ? seq_assoc, ? union_assoc.
+  refl.
+Qed.
+
+Definition sim_local_vwm ex :=
+  ⦗ex.(Execution.label_is) (Label.is_write)⦘ ⨾ Execution.po.
+
+Lemma sim_local_vwm_step ex:
+  sim_local_vwm ex =
+  (sim_local_vwm ex ∪ ⦗ex.(Execution.label_is) (Label.is_write)⦘) ⨾
+  Execution.po_adj.
+Proof.
+  unfold sim_local_vwm. rewrite ? (union_seq' Execution.po_adj), ? seq_assoc, ? union_assoc.
+  rewrite Execution.po_po_adj at 1.
+  rewrite (clos_refl_union Execution.po), union_seq, eq_seq.
+  rewrite ? (seq_union' (Execution.po ⨾ Execution.po_adj) Execution.po_adj), ? seq_assoc, ? union_assoc.
+  refl.
+Qed.
+
+Definition sim_local_vcap ex :=
+  ex.(Execution.ctrl) ∪ (ex.(Execution.addr) ⨾ Execution.po).
+
+Lemma sim_local_vcap_po
+      p ex
+      (EX: Valid.ex p ex):
+  (sim_local_vcap ex ⨾ Execution.po) ⊆ sim_local_vcap ex.
+Proof.
+  unfold sim_local_vcap. ii. inv H. des. inv H0.
+  - left. eapply Valid.ctrl_po; eauto. econs. splits; eauto.
+  - right. inv H. des. econs. splits; eauto. etrans; eauto.
+Qed.
+
+Lemma sim_local_vcap_po_adj
+      p ex
+      (EX: Valid.ex p ex):
+  (sim_local_vcap ex ⨾ Execution.po_adj) ⊆ sim_local_vcap ex.
+Proof.
+  ii. eapply sim_local_vcap_po; eauto.
+  inv H. des. econs. splits; eauto. apply Execution.po_adj_po. ss.
+Qed.
+
+Definition sim_local_vrel ex :=
+  ⦗ex.(Execution.label_is) (Label.is_release)⦘ ⨾ Execution.po.
+
+Lemma sim_local_vrel_step ex:
+  sim_local_vrel ex =
+  (sim_local_vrel ex ∪ ⦗ex.(Execution.label_is) (Label.is_release)⦘) ⨾
+  Execution.po_adj.
+Proof.
+  unfold sim_local_vrel. rewrite ? (union_seq' Execution.po_adj), ? seq_assoc, ? union_assoc.
+  rewrite Execution.po_po_adj at 1.
+  rewrite (clos_refl_union Execution.po), union_seq, eq_seq.
+  rewrite ? (seq_union' (Execution.po ⨾ Execution.po_adj) Execution.po_adj), ? seq_assoc, ? union_assoc.
+  refl.
+Qed.
+
+Lemma sim_local_vrel_spec
+      p ex eid1 eid2
+      (EX: Valid.ex p ex)
+      (EID2: Execution.label_is ex Label.is_acquire eid2)
+      (VREL: sim_local_vrel ex eid1 eid2):
+  <<OB: ex.(Execution.ob) eid1 eid2>>.
+Proof.
+  inv EID2. destruct l; inv LABEL. unfold sim_local_vrel in VREL.
+  right. left. left. left. right.
+  rewrite seq_assoc. econs. splits; eauto. econs; eauto.
+Qed.
+
+Inductive sim_local_fwd ex (loc:Loc.t) (eid1 eid2:eidT): Prop :=
+| sim_local_fwd_intro
+    (PO: Execution.po eid1 eid2)
+    (WRITE: ex.(Execution.label_is) (Label.is_writing loc) eid1)
+    (NWRITE: forall eid
+               (PO: Execution.po eid1 eid)
+               (PO: Execution.po eid eid2),
+        ex.(Execution.label_is) (fun l => ~ Label.is_writing loc l) eid)
+.
+
+Lemma sim_local_fwd_step ex loc:
+  sim_local_fwd ex loc =
+  (sim_local_fwd ex loc ⨾ ⦗ex.(Execution.label_is) (fun l => ~ (Label.is_writing loc l))⦘ ∪
+   ⦗ex.(Execution.label_is) (Label.is_writing loc)⦘) ⨾
+  Execution.po_adj.
+Proof.
+  funext. i. funext. i. propext. econs.
+  - i. inv H. rewrite Execution.po_po_adj in PO. inv PO. des.
+    inv H0. destruct x0, x1. ss. subst.
+    econs. splits; cycle 1.
+    { instantiate (1 := (_, _)). econs; ss. }
+    inv H.
+    + right. econs; ss.
+    + hexploit NWRITE; eauto. i.
+      left. econs. splits; cycle 1.
+      { econs; eauto. }
+      econs; eauto. i. apply NWRITE; eauto. etrans; eauto.
+  - i. inv H. des. inv H1. destruct x0, x1. ss. subst. inv H0.
+    + inv H. des. inv H1. inv H2. inv H0.
+      econs; eauto.
+      * etrans; eauto.
+      * i. rewrite Execution.po_po_adj in PO1. inv PO1. des. inv H0. destruct x0. ss. inv N.
+        inv H; eauto.
+    + inv H. inv H1. apply Label.is_writing_inv in LABEL. des. subst.
+      econs; eauto.
+      * econs; eauto. apply Label.write_is_writing.
+      * i. inv PO. inv PO0. ss. subst. lia.
+Qed.
+
+Lemma sim_local_fwd_functional ex loc eid1 eid2 eid3
+      (EID1: sim_local_fwd ex loc eid1 eid3)
+      (EID2: sim_local_fwd ex loc eid2 eid3):
+  eid1 = eid2.
+Proof.
+  inv EID1. inv EID2.
+  destruct eid1, eid2, eid3. inv PO. inv PO0. ss. subst. f_equal.
+  destruct (Nat.compare_spec n n0); ss.
+  - exploit (NWRITE (t1, n0)); eauto. i.
+    inv WRITE0. apply Label.is_writing_inv in LABEL. des. subst.
+    inv x0. rewrite EID in EID0. inv EID0. ss. destruct (equiv_dec loc loc); ss. congr.
+  - exploit (NWRITE0 (t1, n)); eauto. i.
+    inv WRITE. apply Label.is_writing_inv in LABEL. des. subst.
+    inv x0. rewrite EID in EID0. inv EID0. ss. destruct (equiv_dec loc loc); ss. congr.
+Qed.
+
+Lemma rfi_sim_local_fwd
+      p ex (EX: Valid.ex p ex)
+      loc eid1 eid2
+      (EID1: ex.(Execution.label_is) (Label.is_writing loc) eid1)
+      (EID2: ex.(Execution.label_is) (Label.is_reading loc) eid2)
+      (RFI: ex.(Execution.rfi) eid1 eid2):
+  sim_local_fwd ex loc eid1 eid2.
+Proof.
+  destruct eid1 as [tid1 n1].
+  destruct eid2 as [tid2 n2].
+  inv RFI. inv H0. ss. subst.
+  destruct (Nat.compare_spec n1 n2).
+  - subst. exfalso. eapply EX.(Valid.INTERNAL).
+    econs. right. eauto.
+  - econs; ss. i. destruct eid. inv PO. inv PO0. ss. subst.
+    inv EID1. apply Label.is_writing_inv in LABEL. des. subst.
+    inv EID2. apply Label.is_reading_inv in LABEL. des. subst.
+    exploit Valid.po_label; eauto.
+    { instantiate (1 := (t, n)). econs; ss. }
+    i. des. econs; eauto. intro X. apply Label.is_writing_inv in X. des. subst.
+    exploit Valid.coherence_ww.
+    { eauto. }
+    { econs; try exact EID; eauto. apply Label.write_is_writing. }
+    { econs; try exact LABEL; eauto. apply Label.write_is_writing. }
+    { econs; ss. }
+    i.
+    exploit Valid.coherence_wr; try exact H; eauto.
+    { econs; try exact LABEL; eauto. apply Label.write_is_writing. }
+    { econs; try exact EID0; eauto. apply Label.read_is_reading. }
+    { econs; ss. }
+    i. des.
+    exploit EX.(Valid.RF_WF); [exact H|exact RF|]. i. subst.
+    inv CO.
+    + inv H1. lia.
+    + exfalso. eapply EX.(Valid.INTERNAL). econs 2; econs; left; right; eauto.
+  - exfalso. eapply EX.(Valid.INTERNAL). econs 2; [econs|econs].
+    + right. eauto.
+    + left. left. left. econs; eauto.
+      inv EID1. apply Label.is_writing_inv in LABEL. des. subst.
+      inv EID2. apply Label.is_reading_inv in LABEL. des. subst.
+      econs; eauto. econs; eauto using Label.read_is_accessing, Label.write_is_accessing.
+Qed.
+
+Definition sim_local_fwd_none ex loc :=
+  ⦗ex.(Execution.label_is) (Label.is_writing loc)⦘ ⨾ Execution.po.
+
+Lemma sim_local_fwd_none_step ex loc:
+  sim_local_fwd_none ex loc =
+  (sim_local_fwd_none ex loc ∪ ⦗ex.(Execution.label_is) (Label.is_writing loc)⦘) ⨾
+  Execution.po_adj.
+Proof.
+  unfold sim_local_fwd_none. rewrite ? (union_seq' Execution.po_adj), ? seq_assoc, ? union_assoc.
+  rewrite Execution.po_po_adj at 1.
+  rewrite (clos_refl_union Execution.po), union_seq, eq_seq.
+  rewrite ? (seq_union' (Execution.po ⨾ Execution.po_adj) Execution.po_adj), ? seq_assoc, ? union_assoc.
+  refl.
+Qed.
+
+Definition promises_from_mem
+           (tid:Id.t) (mem: Memory.t): Promises.t.
+Proof.
+  induction mem using list_rev_rect.
+  - exact bot.
+  - destruct x.
+    apply (if tid0 == tid
+           then Promises.set (S (List.length (List.rev mem))) IHmem
+           else IHmem).
+Defined.
+
+Lemma promises_from_mem_nil tid:
+  promises_from_mem tid Memory.empty = bot.
+Proof.
+  unfold promises_from_mem, list_rev_rect, eq_rect. ss.
+  match goal with
+  | [|- context[match ?c with | eq_refl => _ end]] => destruct c
+  end; ss.
+Qed.
+
+Lemma promises_from_mem_snoc tid mem msg:
+  promises_from_mem tid (mem ++ [msg]) =
+  if msg.(Msg.tid) == tid
+  then Promises.set (S (List.length mem)) (promises_from_mem tid mem)
+  else promises_from_mem tid mem.
+Proof.
+  unfold promises_from_mem at 1, list_rev_rect, eq_rect.
+  match goal with
+  | [|- context[match ?c with | eq_refl => _ end]] => destruct c
+  end; ss.
+  rewrite List.rev_involutive, List.rev_app_distr. ss.
+  destruct msg. s. condtac.
+  - inversion e. subst. rewrite ? List.rev_length.
+    f_equal.
+    unfold promises_from_mem, list_rev_rect, eq_rect.
+    match goal with
+    | [|- context[match ?c with | eq_refl => _ end]] => destruct c
+    end; ss.
+  - unfold promises_from_mem, list_rev_rect, eq_rect.
+    match goal with
+    | [|- context[match ?c with | eq_refl => _ end]] => destruct c
+    end; ss.
+Qed.
+
+Lemma promises_from_mem_inv
+      ts tid mem
+      (LOOKUP: Promises.lookup (S ts) (promises_from_mem tid mem)):
+  exists loc val, List.nth_error mem ts = Some (Msg.mk loc val tid).
+Proof.
+  revert LOOKUP. induction mem using List.rev_ind.
+  { rewrite promises_from_mem_nil, Promises.lookup_bot. ss. }
+  rewrite promises_from_mem_snoc. condtac.
+  { rewrite Promises.set_o. condtac.
+    - inversion e. inversion e0. subst.
+      rewrite List.nth_error_app2; [|lia].
+      rewrite Nat.sub_diag. ss.
+      destruct x. esplits; eauto.
+    - i. exploit IHmem; eauto.  i. des.
+      rewrite List.nth_error_app1; eauto.
+      apply List.nth_error_Some. congr.
+  }
+  i. exploit IHmem; eauto.  i. des.
+  rewrite List.nth_error_app1; eauto.
+  apply List.nth_error_Some. congr.
+Qed.
+
+Definition init_with_promises (p:program) (mem:Memory.t): Machine.t :=
+  Machine.mk
+    (IdMap.mapi (fun tid stmts =>
+                   (State.init stmts,
+                    Local.init_with_promises (promises_from_mem tid mem)))
+                p)
+    mem.
+
+Lemma pf_init_with_promises
+      p promises
+      (MEM: forall msg (MSG: List.In msg promises), IdMap.find msg.(Msg.tid) p <> None):
+  exists m,
+    <<STEP: rtc (Machine.step ExecUnit.promise_step) (Machine.init p) m>> /\
+    <<TPOOL: IdMap.Equal m.(Machine.tpool) (init_with_promises p promises).(Machine.tpool)>> /\
+    <<MEM: m.(Machine.mem) = promises>>.
+Proof.
+  revert MEM. induction promises using List.rev_ind; i.
+  { esplits; eauto. ii. s. rewrite IdMap.map_spec, IdMap.mapi_spec.
+    destruct (IdMap.find y p); ss.
+    unfold Local.init, Local.init_with_promises. repeat f_equal.
+    rewrite promises_from_mem_nil. ss.
+  }
+  exploit IHpromises; eauto.
+  { i. apply MEM. apply List.in_app_iff. intuition. }
+  i. des. subst. destruct x.
+  hexploit MEM.
+  { apply List.in_app_iff. right. left. eauto. }
+  match goal with
+  | [|- context[(?f <> None) -> _]] => destruct f eqn:FIND
+  end; ss.
+  intro X. clear X.
+  eexists (Machine.mk _ _). esplits.
+  - etrans; [eauto|]. econs 2; [|refl].
+    econs.
+    + rewrite TPOOL, IdMap.mapi_spec, FIND. ss.
+    + econs; ss. econs; eauto. ss.
+    + ss.
+  - s. ii. rewrite IdMap.add_spec. condtac; ss.
+    + inversion e. subst. rewrite IdMap.mapi_spec, FIND. s.
+      unfold Local.init_with_promises. repeat f_equal.
+      rewrite promises_from_mem_snoc. condtac; ss.
+    + rewrite TPOOL, ? IdMap.mapi_spec. destruct (IdMap.find y p); ss.
+      unfold Local.init_with_promises. rewrite promises_from_mem_snoc. s.
+      condtac; ss. congr.
+  - ss.
+Qed.
+
+(* TODO: move *)
+Lemma step_get_msg_tpool
+      p m ts msg
+      (STEPS: rtc (Machine.step ExecUnit.step) (Machine.init p) m)
+      (MSG: Memory.get_msg ts m.(Machine.mem) = Some msg):
+  exists sl, IdMap.find msg.(Msg.tid) m.(Machine.tpool) = Some sl.
+Proof.
+  apply clos_rt_rt1n_iff in STEPS.
+  apply clos_rt_rtn1_iff in STEPS.
+  revert ts msg MSG. induction STEPS; ss.
+  { destruct ts; ss. destruct ts; ss. }
+  destruct y as [tpool1 mem1].
+  destruct z as [tpool2 mem2].
+  ss. inv H. ss. i. inv STEP.
+  - rewrite IdMap.add_spec. condtac; eauto.
+    inv STEP0. inv STEP. ss. subst. eauto.
+  - rewrite IdMap.add_spec. condtac; eauto.
+    inv STEP0. ss. subst. inv LOCAL. inv MEM2.
+    apply Memory.get_msg_snoc_inv in MSG. des; eauto. subst.
+    ss. congr.
+Qed.
+
+(* TODO: move *)
+Lemma rtc_promise_step_spec
+      p m
+      (STEP: rtc (Machine.step ExecUnit.promise_step) (Machine.init p) m):
+  IdMap.Equal m.(Machine.tpool) (init_with_promises p m.(Machine.mem)).(Machine.tpool).
+Proof.
+  apply clos_rt_rt1n_iff in STEP.
+  apply clos_rt_rtn1_iff in STEP.
+  induction STEP.
+  { s. ii. rewrite IdMap.map_spec, IdMap.mapi_spec.
+    destruct (IdMap.find y p); ss. f_equal. f_equal.
+    rewrite promises_from_mem_nil. ss.
+  }
+  destruct y as [tpool2 mem2].
+  destruct z as [tpool3 mem3].
+  ss. inv H. inv STEP0. inv LOCAL. ss. subst. inv MEM2.
+  ii. generalize (IHSTEP y). rewrite IdMap.add_spec, ? IdMap.mapi_spec.
+  rewrite promises_from_mem_snoc. s.
+  repeat condtac; try congr.
+  inversion e. subst. rewrite FIND. destruct (IdMap.find tid p); ss. i. inv H. ss.
+Qed.
